SEARsorts.sml
@@ -1,0 +1,22 @@
+val _ = new_sort "set" [];
+val _ = new_sort "mem" [("A",mk_sort "set" [])];
+val _ = new_sort "rel" [("A",mk_sort "set" []),("B",mk_sort "set" [])]
+val _ = new_sort_infix "rel" "~>"
+
+val set_sort = mk_sort "set" []
+fun mem_sort A = mk_sort "mem" [A]
+fun rel_sort A B = mk_sort "rel" [A,B]
+fun mk_set A = mk_var(A,set_sort)
+fun mk_rel R A B = mk_var(R,rel_sort A B)
+fun mk_mem a A = mk_var(a,mem_sort A)
+
+val _ = EqSorts := "rel" :: (!EqSorts)
+val _ = EqSorts := "mem" :: (!EqSorts)
+
+
+val _ = new_sort "fun" [("A",mk_sort "set" []),("B",mk_sort "set" [])]
+val _ = new_sort_infix "fun" "->"
+
+fun fun_sort A B = mk_sort "fun" [A,B]
+fun mk_func f A B = mk_var(f,fun_sort A B)
+val _ = EqSorts := "fun" :: (!EqSorts)
