SEARsetting.sml
@@ -1,132 +1,4 @@
-val _ = new_sort "set" [];
-val _ = new_sort "mem" [("A",mk_sort "set" [])];
-val _ = new_sort "rel" [("A",mk_sort "set" []),("B",mk_sort "set" [])]
-val _ = new_sort_infix "rel" "~>"
-
-val set_sort = mk_sort "set" []
-fun mem_sort A = mk_sort "mem" [A]
-fun rel_sort A B = mk_sort "rel" [A,B]
-fun mk_set A = mk_var(A,set_sort)
-fun mk_rel R A B = mk_var(R,rel_sort A B)
-fun mk_mem a A = mk_var(a,mem_sort A)
-
-val _ = EqSorts := "rel" :: (!EqSorts)
-val _ = EqSorts := "mem" :: (!EqSorts)
-
-val _ = new_pred "Holds" [("R",rel_sort (mk_set "A") (mk_set "B")),
-                         ("a",mem_sort (mk_set "A")),
-                         ("b",mem_sort (mk_set "B"))]
-
-
 val AX0 = store_ax("AX0",“?A a:mem(A).T”);
-
-val AX1 = store_ax("AX1",
-“!A B:set.?!R:A~>B.!a:mem(A) b:mem(B).Holds(R,a,b)<=> P(a,b)”);
-
-val Fun_def = 
-    qdefine_psym ("isFun",[‘R:A~>B’]) 
-                 ‘!x:mem(A). ?!y:mem(B). Holds(R,x,y)’
-    |> gen_all |> store_as "Fun_def";
-
-
-val Fun_expand = proved_th $
-e0
-(rpt strip_tac >> rw[Fun_def] >>
- rw[uex_def “?!y:mem(B).Holds(R,x,y)”] >> 
- dimp_tac >> strip_tac (* 2 *)
- >-- (rpt strip_tac (* 2 *)
-     >-- (first_x_assum (qspecl_then [‘a’] assume_tac) >> 
-          pop_assum strip_assume_tac >> qexists_tac ‘y’ >> arw[]) 
-     >-- (first_x_assum (qspecl_then [‘a’] strip_assume_tac) >>
-          first_assum rev_drule >>
-          first_assum (qspecl_then [‘b2’] assume_tac) >>
-          first_assum drule >> arw[])) >>
- rpt strip_tac >> last_x_assum (qspecl_then [‘x’] strip_assume_tac) >>
- qexists_tac ‘b’ >> arw[] >> rpt strip_tac >> first_x_assum irule >>
- qexists_tac ‘x’ >> arw[])
-(form_goal
-“!A B R:A~>B. isFun(R) <=>
- (!a.?b.Holds(R,a,b)) & 
- (!a b1 b2. Holds(R,a,b1) & Holds(R,a,b2) ==> b1 = b2)”)
-
-
-(*
-val Fun_expand = proved_th $
-e0
-(rpt strip_tac >> rw[Fun_def] >>
- rw[uex_def “?!y:mem(B).Holds(R,x,y)”] >> 
- dimp_tac >> strip_tac (* 2 *)
- >-- (rpt strip_tac (* 2 *)
-     >-- (first_x_assum (qspecl_then [‘a’] assume_tac) >> 
-          pop_assum strip_assume_tac >> qexists_tac ‘y’ >> arw[]) 
-     >-- (first_x_assum (qspecl_then [‘a’] strip_assume_tac) >>
-          first_assum rev_drule >>
-          first_assum (qspecl_then [‘b2’] assume_tac) >>
-          first_assum drule >> arw[])) >>
- rpt strip_tac >> last_x_assum (qspecl_then [‘x’] strip_assume_tac) >>
- qexists_tac ‘b’ >> arw[] >> rpt strip_tac >-- rw[] >> first_x_assum irule >>
- qexists_tac ‘x’ >> arw[])
-(form_goal
-“!A B R:A~>B. isFun(R) <=>
- (!a.?b.Holds(R,a,b)) & 
- (!a b1 b2. Holds(R,a,b1) & Holds(R,a,b2) ==> b1 = b2)”)
-*)
-
-val _ = new_sort "fun" [("A",mk_sort "set" []),("B",mk_sort "set" [])]
-val _ = new_sort_infix "fun" "->"
-
-fun fun_sort A B = mk_sort "fun" [A,B]
-fun mk_func f A B = mk_var(f,fun_sort A B)
-val _ = EqSorts := "fun" :: (!EqSorts)
-
-val _ = new_fun "App" (mem_sort (mk_set "B"),
-                       [("f",fun_sort (mk_set "A") (mk_set "B")),
-                       ("a",mem_sort (mk_set "A"))]);
-
-val rel2fun = store_ax("rel2fun",
-“!A B R:A~>B. isFun(R) ==> ?!f:A->B. !a b. App(f,a) = b <=> Holds(R,a,b)”);
-
-
-local
-val l = fVar_sInst_th
-“P(a:mem(A),b:mem(B))”
-“App(f:A->B,a) = b”
-(AX1 |> qspecl [‘A’, ‘B’] |> uex_expand)
-in
-val asR_ex = prove_store("asR_ex",
-e0
-(rpt strip_tac >> strip_assume_tac l >>
- qexists_tac ‘R’ >> arw[])
-(form_goal
- “!A B f:A->B.?R.!a b. Holds(R,a,b) <=> App(f,a) = b”));
-end
- 
-val exth = proved_th $
-e0
-(strip_tac >> 
- qsspecl_then [‘f’] strip_assume_tac asR_ex >>
- qexists_tac ‘R’ >> rw[])
-(form_goal “!f:A->B.?R:A~>B.T”)
-
-val asR_def = asR_ex |> spec_all |> SKOLEM (spec_all exth) "asR"
-                     [dest_var (rastt "f:A -> B")]
-
-val Inj_def = 
-    qdefine_psym ("Inj",[‘f:A->B’]) 
-                 ‘!x1 x2. App(f,x1) = App(f,x2) ==> x1 = x2’
-    |> gen_all |> store_as "Inj_def";
-
-val Surj_def = 
-    qdefine_psym ("Surj",[‘f:A->B’]) 
-                 ‘!b. ?a. App(f,a) = b’
-    |> gen_all |> store_as "Surj_def";
- 
-val Bij_def =
-    qdefine_psym ("Bij",[‘f:A->B’]) 
-                 ‘Inj(f) & Surj(f)’
-    |> gen_all |> store_as "Bij_def";
-
-
 
 val _ = new_pred "isTab" [("R",rel_sort (mk_set "A") (mk_set "B")),
                           ("p",rel_sort (mk_set "TR") (mk_set "A")),
@@ -143,8 +15,6 @@ val Tab_def = qdefine_psym ("isTab",[‘R:A~>B’,‘p:TR -> A’,‘q:TR->B’]
 val AX2 = new_ax “!A B R:A~>B.?TR p:TR->A q:TR->B. 
 (!x y. Holds(R,x,y) <=> ?r. App(p,r) = x & App(q,r) = y) & 
  !r s. App(p,r) = App(p,s) & App(q,r) = App(q,s) ==> r = s”;
-
-
 
 local
 val lemma = 
@@ -168,6 +38,33 @@ e0
 “?Empty. !a:mem(Empty).F”));
 end
  
+
+val Empty_unique = prove_store("Empty_unique",
+e0
+(rpt strip_tac >>
+ strip_assume_tac
+ (AX1_ex |> qspecl [‘E1’,‘E2’] 
+         |> fVar_sInst_th “P(a:mem(E1),b:mem(E2))” “F”) >>
+ strip_assume_tac
+ (AX1_ex |> qspecl [‘E2’,‘E1’] 
+         |> fVar_sInst_th “P(a:mem(E2),b:mem(E1))” “F”) >>
+ qby_tac ‘isFun(R)’
+ >-- (rw[Fun_def] >> strip_tac >> 
+ last_x_assum (qspecl_then [‘x’] assume_tac) >> fs[]) >>
+ qby_tac ‘isFun(R')’
+ >-- (rw[Fun_def] >> strip_tac >> 
+ last_x_assum (qspecl_then [‘x’] assume_tac) >> fs[]) >> 
+ rev_drule rel2fun_ex >> pop_assum strip_assume_tac >>
+ drule rel2fun_ex >> pop_assum strip_assume_tac >> 
+ qexistsl_tac [‘f’,‘f'’] >> 
+ arw[GSYM FUN_EXT] >> rpt strip_tac (* 2 *)
+ >-- (last_x_assum (qspecl_then [‘a’] assume_tac) >> fs[]) >>
+ last_x_assum (qspecl_then [‘a’] assume_tac) >> fs[])
+(form_goal
+ “∀E1 E2. (!a:mem(E1).F) ∧ (!a:mem(E2).F) ⇒
+  ∃i:E1->E2 j:E2->E1. i o j = Id(E2) ∧ j o i = Id(E1)”));
+
+
 local 
 val lemma = 
     AX1 |> qspecl [‘A’,‘A’]
@@ -191,69 +88,114 @@ e0
 “?ONE x:mem(ONE). !x':mem(ONE). x' = x”));
 end
 
-local
-val exth = proved_th $
+
+val unique_fun_to_ONE = prove_store("unique_fun_to_ONE",
 e0
-(strip_assume_tac Thm_2_3 >> qexists_tac ‘ONE’ >> rw[])
-(form_goal “?a:set.T”)
-in
-val ONE_def = SKOLEM exth "1" [] Thm_2_3
-end
+(rpt strip_tac >>
+ uex_tac >> 
+ assume_tac (qfun_compr ‘a:mem(A)’ ‘x:mem(ONE)’) >>
+ pop_assum (strip_assume_tac o uex_expand) >>
+ qexists_tac ‘f’ >> arw[GSYM FUN_EXT])
+(form_goal “∀ONE x:mem(ONE). (∀a. a = x) ==> 
+ ∀A. ?!f:A->ONE. T”));
+
+val ONE_unique = prove_store("ONE_unique",
+e0
+(rpt strip_tac >>
+ drule unique_fun_to_ONE >> 
+ first_assum (qspecl_then [‘ONE’] (strip_assume_tac o uex_expand)) >>
+ first_assum (qspecl_then [‘ONE'’] (strip_assume_tac o uex_expand)) >>
+ rev_drule unique_fun_to_ONE >>
+ first_assum (qspecl_then [‘ONE'’] ((x_choose_then "g" strip_assume_tac) o 
+                                   uex_expand)) >>
+ first_assum (qspecl_then [‘ONE’] ((x_choose_then "g'" strip_assume_tac) o 
+                                   uex_expand))  >>
+ qexistsl_tac [‘f’,‘g’] >> strip_tac (* 2 *) >--
+ (first_assum (qspecl_then [‘f o g’] assume_tac) >>
+ first_assum (qspecl_then [‘Id(ONE')’] assume_tac) >> fs[]) >>
+first_assum (qspecl_then [‘g o f’] assume_tac) >>
+ first_assum (qspecl_then [‘Id(ONE)’] assume_tac) >> fs[])
+(form_goal
+ “∀ONE x ONE' x'. (!a:mem(ONE).a = x) ∧ (!a:mem(ONE').a = x') ⇒
+  ∃i:ONE->ONE' j:ONE'->ONE. 
+  i o j = Id(ONE') ∧ j o i = Id(ONE)”));
+
+
+val iso0_REFL = prove_store("iso0_REFL",
+e0
+(strip_tac >> qexistsl_tac [‘Id(A)’,‘Id(A)’] >> rw[IdL,IdR])
+(form_goal “∀A. ∃i:A->A j. i o j = Id(A) & j o i = Id(A)”));
+
+
+val iso0_SYM = prove_store("iso0_SYM",
+e0
+(rpt strip_tac >> qexistsl_tac [‘j’,‘i’] >> arw[])
+(form_goal 
+ “∀A A'. 
+  (∃i:A->A' j. i o j = Id(A') & j o i = Id(A)) ⇒
+  (∃i:A'->A j. i o j = Id(A) & j o i = Id(A'))”));
+
+
+val iso0_TRANS = prove_store("iso0_SYM",
+e0
+(rpt strip_tac >> qexistsl_tac [‘i' o i’,‘j o j'’] >> arw[] >>
+ qsuff_tac
+ ‘i' o (i o j) o j' = Id(A'') & j o (j' o i') o i = Id(A)’ 
+ >-- rw[o_assoc] >>
+ arw[IdL,IdR])
+(form_goal 
+ “∀A A' A''. 
+  (∃i:A->A' j. i o j = Id(A') & j o i = Id(A)) &
+  (∃i:A'->A'' j. i o j = Id(A'') & j o i = Id(A')) ⇒ 
+  (∃i:A->A'' j. i o j = Id(A'') & j o i = Id(A))”));
+
+val iso_Reqv = conjI iso0_REFL (conjI iso0_SYM iso0_TRANS) 
+
+val ONE_uex = prove_store("ONE_uex",
+e0
+(strip_assume_tac Thm_2_3 >> qexists_tac ‘ONE’ >>
+ rpt strip_tac (* 2 *)
+ >-- (qexists_tac ‘x’ >> arw[]) >>
+ irule ONE_unique >> rpt strip_tac (* 2 *)
+ >-- (qexists_tac ‘x’ >> arw[]) >>
+ qexists_tac ‘x'’ >> arw[])
+(form_goal 
+ “∃ONE. (∃x. (!a:mem(ONE).a = x)) ∧
+ ∀ONE'. (∃x.(!a:mem(ONE').a = x))  ⇒
+  ∃i:ONE->ONE' j:ONE'->ONE. 
+  i o j = Id(ONE') ∧ j o i = Id(ONE)”));
 
 local
-val exth' = proved_th $
+val eth = proved_th $
 e0
-(strip_assume_tac ONE_def >> qexists_tac ‘x’ >> rw[])
-(form_goal “?a:mem(1).T”)
+(strip_assume_tac Thm_2_3 >> qexists_tac ‘ONE’ >> rw[])
+(form_goal “∃ONE. T”)
+val eqvth = iso_Reqv 
 in
-val dot_def = SKOLEM exth' "dot" [] ONE_def
+val ONE_def = new_spec ([("ONE",set_sort)],“∃x.∀a:mem(ONE). a = x”) 
+([("ONE",set_sort)],[("ONE'",set_sort)],
+ “(∃i:ONE->ONE' j. i o j = Id(ONE') & j o i = Id(ONE))”)
+["1"] [] eth eqvth ONE_uex
 end
+
+val dot_uex = prove_store("dot_uex",
+e0
+(strip_assume_tac ONE_def >> uex_tac >> qexists_tac ‘x’ >> arw[] )
+(form_goal “?!x:mem(1).x = x”));
+
+val dot_def0 = qsimple_uex_spec "dot" [] dot_uex 
+
+val dot_def = prove_store("dot_def",
+e0
+(strip_assume_tac (uex_expand dot_uex) >>
+ strip_tac >> 
+ first_assum (qspecl_then [‘dot’] assume_tac) >>
+ first_assum (qspecl_then [‘a’] assume_tac) >> fs[])
+(form_goal “∀a:mem(1). a = dot”));
+
 
 val ONE = mk_fun "1" []
 val dot = mk_fun "dot" []
-
-
-local
-val l = AX1 |> qspecl [‘A’,‘B’] |> uex_expand
-            |> fVar_sInst_th “P(a:mem(A),b:mem(B))”
-            “Holds(R1:A~>B,a,b)” 
-in
-val R_EXT = prove_store("R_EXT",
-e0
-(rpt strip_tac >> dimp_tac >> rpt strip_tac >> arw[] >>
- strip_assume_tac l >>
- qsuff_tac ‘R1 = R & R2= R’ >-- (strip_tac >> arw[]) >> 
- strip_tac >> first_x_assum irule >> arw[]
- )
-(form_goal
-“!A B R1:A~>B R2. (!a b.Holds(R1,a,b) <=> Holds(R2,a,b)) <=> R1= R2”));
-end
-
-
-val asR_Fun = prove_store("asR_Fun",
-e0
-(rpt strip_tac >> rw[Fun_expand] >>
- rw[asR_def] >> rpt strip_tac (* 2 *)
- >-- (qexists_tac ‘App(f,a)’ >> rw[]) >>
- pop_assum (assume_tac o GSYM) >> arw[])
-(form_goal
- “!A B f:A->B. isFun(asR(f))”));
-
-
-val FUN_EXT = prove_store("FUN_EXT",
-e0
-(rpt strip_tac >> 
- assume_tac rel2fun >>
- first_x_assum (qsspecl_then [‘asR(f2)’] assume_tac) >>
- qsspecl_then [‘f2’] assume_tac asR_Fun >>
- first_x_assum drule >>
- pop_assum (strip_assume_tac o uex_expand) >>
- dimp_tac >> rpt strip_tac >> arw[] >>
- qsuff_tac ‘f1 = f & f2 = f’ 
- >-- (strip_tac >> arw[]) >> strip_tac >> first_x_assum irule (* 2 *) >>
- arw[asR_def])
-(form_goal “!A B f1:A->B f2. 
- (!a.App(f1,a) = App(f2,a)) <=> f1 = f2”));
 
 
 local 
@@ -279,12 +221,15 @@ e0
 “!A.?!f:A~>1. isFun(f)”));
 end
 
+(*
+
 val asR_eq_eq = prove_store("asR_eq_eq",
 e0
 (rpt strip_tac >> dimp_tac >> rpt strip_tac >> arw[] >>
  irule $ iffLR FUN_EXT >> 
  drule $ iffRL R_EXT >> fs[asR_def])
 (form_goal “!A B f1:A->B f2. asR(f1) = asR(f2) <=> f1 = f2”));
+*)
 
 val To1_ex = prove_store("To1_ex",
 e0
@@ -304,11 +249,24 @@ e0
 (form_goal “!A. ?!f:A ->1. T”));
 
 
- 
-val To1_def = SKOLEM (To1_ex |> spec_all |> uex2ex_rule) 
-                     "To1" [dest_var $ rastt "A"] 
-                     (To1_ex |> spec_all |> uex_expand)
-                     |> rewr_rule []
+val To1_uex = prove_store("To1_uex",
+e0
+(rw[To1_ex])
+(form_goal “!A. ?!f:A ->1. f = f”));
+
+
+(*{(A : set)},  |- !(f' : fun(A, 1)). f'# = To1(A): thm*)
+val To1_def0 =  qsimple_uex_spec "To1" [‘A’] (spec_all To1_uex)
+
+val To1_def =  prove_store("To1_def",
+e0
+(strip_tac >>
+ qspecl_then [‘A’] (strip_assume_tac o uex_expand) To1_uex >>
+ strip_tac >>
+ first_assum (qspecl_then [‘f'’] assume_tac) >>
+ first_assum (qspecl_then [‘To1(A)’] assume_tac) >> fs[])
+(form_goal “!A f:A->1. f = To1(A)”));
+
 
 
 val Thm_2_4_R_ver = prove_store("Thm_2_4_R_ver",
@@ -430,187 +388,6 @@ e0
 “!A B R:A~>B T1 p1:T1->A q1:T1->B T2 p2:T2->A q2:T2->B.
  isTab(R,p1,q1) & isTab(R,p2,q2) ==> ?b:T1->T2. Bij(b)”)
 end
-
-val _ = new_fun "@" (rel_sort (mk_set "A") (mk_set "C"),
-                     [("phi",rel_sort (mk_set "B") (mk_set "C")),
-                      ("psi",rel_sort (mk_set "A") (mk_set "B"))])
-
-val ao_def = store_ax("ao_def",
-“!A B phi:A~>B C psi:B~>C a:mem(A) c:mem(C). 
-(?b. Holds(phi,a,b) & Holds(psi,b,c)) <=> Holds(psi @ phi,a,c)”);
-
-val _ = new_fun "id" (rel_sort (mk_set "A") (mk_set "A"),
-                     [("A",set_sort)])
-
-val id_def = store_ax("id_def",“!A a:mem(A) b. Holds(id(A),a,b) <=> a = b”);
-
-val id_Fun = prove_store("id_Fun",
-e0
-(strip_tac >> rw[Fun_expand,id_def] >> flip_tac >> rpt strip_tac
- >-- (qexists_tac ‘a’ >> rw[]) >>
- pop_assum (assume_tac o GSYM) >> arw[])
-(form_goal
- “!A. isFun(id(A))”));
-
-
-val idL = prove_store("idL",
-e0
-(rpt strip_tac >> irule $ iffLR R_EXT >> 
- rw[GSYM ao_def,id_def] >> rpt strip_tac >> dimp_tac >> strip_tac
- >-- fs[] >> qexists_tac ‘b’ >> arw[])
-(form_goal
- “!A B f:A~>B. id(B) @ f = f”));
-
-
-val idR = prove_store("idR",
-e0
-(rpt strip_tac >> irule $ iffLR R_EXT >> 
- rw[GSYM ao_def,id_def] >> rpt strip_tac >> dimp_tac >> strip_tac
- >-- fs[] >> qexists_tac ‘a’ >> arw[])
-(form_goal
- “!A B f:A~>B. f @ id(A) = f”));
- 
-
-val Id_ex = prove_store("Id_ex",
-e0
-(strip_tac >>
- qspecl_then [‘A’] assume_tac id_Fun >>
- drule rel2fun >>
- pop_assum (strip_assume_tac o uex_expand) >>
- qexists_tac ‘f’  >> arw[id_def])
-(form_goal “!A. ?i:A ->A. (!a.App(i,a) = a)”));
-
-val Id_def = qSKOLEM "Id" [‘A’] (Id_ex|> spec_all) 
-                     |> gen_all |> store_as "Id_def";
-
-val App_Id = Id_def |> store_as "App_Id";
-
-val Thm_2_7_assoc = proved_th $
-e0
-(rpt strip_tac >> once_rw[GSYM R_EXT] >> rw[GSYM ao_def] >> rpt strip_tac >>
- dimp_tac >> rpt strip_tac (* 2 *)
- >-- (qexists_tac ‘b''’ >> arw[] >> qexists_tac ‘b'’ >> arw[]) >>
- qexists_tac ‘b''’ >> arw[] >> qexists_tac ‘b'’ >> arw[])
-(form_goal
-“!A B phi:A~>B C psi:B~>C D chi:C~>D. (chi @ psi) @ phi = chi @ psi @ phi”)
-
-val Thm_2_7_id = proved_th $
-e0
-(rpt strip_tac >> rw[GSYM R_EXT] >> rpt strip_tac  (* 2 *)
- >-- (rw[GSYM ao_def,id_def] >> dimp_tac >> rpt strip_tac
-      >-- arw[] >> qexists_tac ‘a’ >> arw[]) >>
- rw[GSYM ao_def,id_def] >> dimp_tac >> rpt strip_tac 
- >-- fs[] >> qexists_tac ‘b’ >> arw[])
-(form_goal
-“!A B phi:A~>B. phi @ id(A) = phi & id(B) @ phi = phi”)
-
-val _ = new_fun "op" (rel_sort (mk_set "B") (mk_set "A"),[("R",rel_sort (mk_set "A") (mk_set "B"))])
-
-val op_def = store_ax("op_def",“!A B R:A~>B a b.Holds(op(R),a,b) <=> Holds(R,b,a)”);
-
-
-val Thm_2_7_ao_Fun = prove_store("Thm_2_7_ao_Fun",
-e0
-(rpt strip_tac >> fs[Fun_expand,GSYM ao_def] >> rpt strip_tac (* 2 *)
- >-- (last_x_assum (qspecl_then [‘a’] strip_assume_tac) >>
-      last_x_assum (qspecl_then [‘b’] strip_assume_tac) >>
-      qexistsl_tac [‘b'’,‘b’] >> arw[]) >>
- first_x_assum irule >> 
- qby_tac ‘b' = b’ >--
- (first_x_assum irule >> qexistsl_tac [‘a’] >> arw[]) >>
- fs[] >> qexists_tac ‘b’ >> arw[])
-(form_goal
- “!A B f:A~>B C g:B~>C. isFun(f) & isFun(g) ==> isFun(g @ f)”));
-
-val ao_Fun = Thm_2_7_ao_Fun |> store_as "ao_Fun";  
-
-
-val o_ex = prove_store("o_ex",
-e0
-(rpt strip_tac >> 
- qsspecl_then [‘phi’] assume_tac asR_Fun >>
- qsspecl_then [‘psi’] assume_tac asR_Fun >>
- qby_tac ‘isFun(asR(psi) @ asR(phi))’ 
- >-- (irule ao_Fun >> arw[]) >>
- drule rel2fun >>
- pop_assum (strip_assume_tac o uex_expand) >>
- qexists_tac ‘f’ >> arw[])
-(form_goal
- “!A B phi:A->B C psi:B->C. ?f:A->C. 
- !a c. App(f,a) = c <=> Holds(asR(psi) @ asR(phi),a,c)”));
-
-val o_def = qSKOLEM "o" [‘psi:B->C’,‘phi:A->B’] 
-                        (o_ex |> spec_all)
-                        |> gen_all |> store_as "o_def";
-
-
-val Bij_op = prove_store("Bij_op",
-e0
-(rpt strip_tac >>
- qsuff_tac ‘isFun(op(asR(f)))’ 
- >-- (strip_tac >> drule rel2fun >>
-     pop_assum (strip_assume_tac o uex_expand) >>
-     qexists_tac ‘f'’ >>
-     arw[GSYM R_EXT,asR_def,op_def]) >> 
- rw[Fun_expand] >>
- fs[Bij_def,Inj_def,Surj_def] >> rpt strip_tac (* 2 *)
- >-- (first_x_assum (qspecl_then [‘a’] strip_assume_tac) >>
-      qexists_tac ‘a'’ >> arw[op_def,asR_def]) >>
- fs[op_def,asR_def] >> first_x_assum irule >> arw[])
-(form_goal “!A B f:A->B. Bij(f) ==> 
- ?f':B->A. asR(f') = op(asR(f))”))
-
-
-val App_App_o = prove_store("App_App_o",
-e0
-(rw[o_def,GSYM ao_def,asR_def] >> rpt strip_tac >>
- qexists_tac ‘App(f,a)’ >> arw[])
-(form_goal “!A B f:A->B C g:B->C a. 
-  App(g o f,a) = App(g,App(f,a))”));
-
-val asR_o = prove_store("asR_o",
-e0
-(rw[GSYM R_EXT,asR_def,GSYM ao_def] >> rpt strip_tac >>
- dimp_tac >> strip_tac (* 2 *)
- >-- (qexists_tac ‘App(f,a)’ >> arw[GSYM App_App_o]) >>
- arw[App_App_o])
-(form_goal “!A B f:A->B C g:B ->C. 
- asR(g o f) = asR(g) @ asR(f)”));
- 
-val asR_Id = prove_store("asR_Id",
-e0
-(rw[asR_def,Id_def,id_def,GSYM R_EXT])
-(form_goal
- “!A. asR(Id(A)) = id(A)”));
-
-
-val Thm_2_7_bij = prove_store("Thm_2_7_bij",
-e0
-(rpt strip_tac >> dimp_tac >> rpt strip_tac (* 2 *)
- >-- (drule Bij_op >> pop_assum strip_assume_tac >>
-     qexists_tac ‘f'’ >> pop_assum mp_tac >>
-     rw[GSYM asR_eq_eq,asR_o,asR_Id,GSYM R_EXT] >>
-     rw[GSYM ao_def,asR_def,id_def,op_def] >>
-     strip_tac >> arw[] >> rpt strip_tac >--
-     (fs[Bij_def,Inj_def] >> dimp_tac >> strip_tac
-      >-- (first_x_assum irule >> arw[]) >>
-      qexists_tac ‘App(phi,a)’ >> arw[]) >>
-     fs[Bij_def,Inj_def,Surj_def] >> 
-     dimp_tac >> strip_tac (* 2 *)
-     >-- (qpick_x_assum ‘App(phi, b') = a’ 
-          (assume_tac o GSYM) >> arw[]) >>
-     arw[] >> 
-     last_x_assum (qspecl_then [‘b’] strip_assume_tac) >>
-     qexists_tac ‘a'’ >> arw[]) >>
- rw[Bij_def,Inj_def,Surj_def] >> rpt strip_tac (* 2 *)
- >-- (qby_tac ‘App(psi,App(phi, x1)) = App(psi,App(phi, x2))’ 
-      >-- arw[] >>
-      rfs[GSYM App_App_o,Id_def]) >>
- qexists_tac ‘App(psi,b)’ >> arw[GSYM App_App_o,Id_def])
-(form_goal
- “!A B phi:A->B.Bij(phi) <=> ?psi:B->A. psi o phi = Id(A) & phi o psi = Id(B)”));
-
-(*val _ = new_fun "*" (set_sort,[("A",set_sort),("B",set_sort)]) *)
 (*
 For sets A and B, let ⊤:A↬B denote the relation such that ⊤(x,y) holds always. A tabulation of ⊤ is denoted A×B; it is a set equipped with functions p:A×B→A and q:A×B→B such that for any x∈A and y∈B, there exists a unique z∈A×B with p(z)=x and q(z)=y. It is called the cartesian product of A and B.
 Theorem 2.8. For any sets A and B, A×B is a product of A and B in the category Set, and a coproduct in the category Rel.
@@ -636,6 +413,79 @@ e0
 (form_goal
 “!A B. ?T0:A~>B. !a b. Holds(T0,a,b)”));
 
+
+val isPair_def = qdefine_psym("isPair",[‘p1:AxB->A’,‘p2:AxB->B’])
+‘!x:mem(A) y:mem(B). 
+   ?!r:mem(AxB).App(p1,r) = x & App(p2,r) = y’
+
+val isPair_uex = prove_store("isPair_uex",
+e0
+(rpt gen_tac >> strip_tac (* 2 *)
+ >-- fs[isPair_def] >>
+     qby_tac
+     ‘∀ab:mem(AB).
+      ?!ab'. App(p1,ab) = App(p1',ab') & 
+             App(p2,ab) = App(p2',ab')’ 
+     >-- (strip_tac >> flip_tac >> arw[]) >>
+     drule
+     (P2fun |> qspecl [‘AB’,‘AB'’] 
+     |> fVar_sInst_th “P(ab:mem(AB),ab':mem(AB'))”
+        “App(p1:AB->A,ab) = App(p1':AB'->A,ab') & 
+         App(p2:AB->B,ab) = App(p2':AB'->B,ab')”) >>
+     pop_assum (x_choose_then "i" assume_tac) >>
+     qby_tac
+     ‘∀ab':mem(AB').
+      ?!ab. App(p1,ab) = App(p1',ab') & 
+             App(p2,ab) = App(p2',ab')’ 
+     >-- arw[] >>
+     drule
+     (P2fun |> qspecl [‘AB'’,‘AB’] 
+     |> fVar_sInst_th “P(ab':mem(AB'),ab:mem(AB))”
+        “App(p1:AB->A,ab) = App(p1':AB'->A,ab') & 
+         App(p2:AB->B,ab) = App(p2':AB'->B,ab')”) >> 
+     pop_assum (x_choose_then "j" assume_tac) >>
+     qexistsl_tac [‘i’,‘j’] >>
+     qby_tac
+     ‘i o j = Id(AB')’ 
+     >-- (arw[GSYM FUN_EXT,Id_def,App_App_o] >>
+         pop_assum (assume_tac o GSYM) >> arw[]) >>
+     qby_tac
+     ‘j o i = Id(AB)’ 
+     >-- (arw[GSYM FUN_EXT,Id_def,App_App_o] >>
+          strip_tac >>
+          last_x_assum (qsspecl_then [‘a’,‘App(i,a)’] (assume_tac o GSYM)) >>
+          arw[]) >>
+     arw[] >>
+     qby_tac
+     ‘p1' o i = p1 & p2' o i = p2’
+     >-- (arw[GSYM FUN_EXT,App_App_o] >> 
+         qpick_x_assum
+         ‘∀a b.
+          App(i, a) = b <=>
+          App(p1, a) = App(p1', b) & App(p2, a) = App(p2', b)’
+         (assume_tac o GSYM) >> flip_tac >> 
+         qsuff_tac
+         ‘∀a. App(p1,a) = App(p1',App(i,a)) &
+              App(p2,a) = App(p2',App(i,a))’ 
+         >-- (rpt strip_tac >> arw[]) >> arw[]) >> arw[] >>
+     arw[GSYM FUN_EXT,App_App_o] >> 
+     qpick_x_assum
+     ‘∀a b.
+      App(j, a) = b <=>
+      App(p1, b) = App(p1', a) & App(p2, b) = App(p2', a)’
+         (assume_tac o GSYM) >> 
+     qsuff_tac
+     ‘∀a. App(p1,App(j,a)) = App(p1',a) &
+          App(p2,App(j,a)) = App(p2',a)’ 
+     >-- (rpt strip_tac >> arw[]) >>
+     arw[])
+(form_goal “!A B AB p1:AB->A p2:AB ->B AB' p1':AB'->A p2'. 
+ isPair(p1,p2) & isPair(p1',p2') ⇒ 
+ ?i:AB->AB' j. i o j = Id(AB') & j o i = Id(AB) &
+  p1' o i = p1 & p2' o i = p2 &
+  p1 o j = p1' & p2 o j = p2'”));
+
+
 val Cross_ex = prove_store("Cross_ex",
 e0
 (rpt strip_tac >> 
@@ -648,21 +498,117 @@ e0
    ?r:mem(AxB).App(p1,r) = x & App(p2,r) = y) &
    !r s. App(p1,r) = App(p1,s) & App(p2,r) = App(p2,s) ==> r = s”)); 
 
+val Pr_uex = prove_store("Pr_uex",
+e0
+(rpt strip_tac >>
+ qspecl_then [‘A’,‘B’] assume_tac Cross_ex >>
+ pop_assum strip_assume_tac >>
+ qexistsl_tac [‘AxB’,‘p1’,‘p2’] >>
+ qby_tac
+ ‘isPair(p1,p2)’ 
+ >-- (rw[isPair_def] >>
+     rpt strip_tac >>
+     uex_tac >> first_x_assum (qspecl_then [‘x’,‘y’] strip_assume_tac) >>
+     qexists_tac ‘r’ >> arw[] >>
+     rpt strip_tac >> first_x_assum irule >> arw[]) >>
+ arw[] >> rpt strip_tac >>
+ qsspecl_then [‘p1’,‘p2’,‘p1'’,‘p2'’] assume_tac  isPair_uex >>
+ first_x_assum irule >> arw[])
+(form_goal “!A B. ?AB p1:AB->A p2:AB ->B. 
+ isPair(p1,p2) &
+ (!AB' p1':AB'->A p2'. isPair(p1',p2') ==>
+  ?i:AB->AB' j. i o j = Id(AB') & j o i = Id(AB) &
+  p1' o i = p1 & p2' o i = p2 &
+  p1 o j = p1' & p2 o j = p2')”));
 
-val Cross_def = Cross_ex |> spec_all 
-                         |> qSKOLEM "*" [‘A’,‘B’]
-                         |> gen_all 
-                         |> store_as "Cross_def"; 
+val Pr_ts_ex = proved_th $
+e0
+(rpt strip_tac >>
+ qspecl_then [‘A’,‘B’] strip_assume_tac Cross_ex >>
+ qexistsl_tac [‘AxB’,‘p1’,‘p2’] >> rw[])
+(form_goal “!A B. ?AB p1:AB->A p2:AB ->B. T”)
 
-val p1_def = Cross_def |> spec_all 
-                       |> qSKOLEM "p1" [‘A’,‘B’]
-                       |> gen_all 
-                       |> store_as "p1_def";
+val isPair_Reqv = proved_th $
+e0
+(rpt strip_tac (* 3 *)
+ >-- (qexistsl_tac [‘Id(AB)’,‘Id(AB)’] >> rw[IdL,IdR]) 
+ >-- (qexistsl_tac [‘j’,‘i’] >> arw[]) >>
+ qexistsl_tac [‘i' o i’,‘j o j'’] >>
+ arw[GSYM o_assoc] >>
+ qsuff_tac
+ ‘i' o (i o j) o j' = Id(AB'') & j o (j' o i') o i = Id(AB)’ 
+ >-- rw[o_assoc] >>
+ arw[IdL,IdR])
+(form_goal 
+“(!AB p1:AB->A p2:AB->B.
+ ?i:AB->AB j. i o j = Id(AB) & j o i = Id(AB) &
+  p1 o i = p1 & p2 o i = p2 &
+  p1 o j = p1 & p2 o j = p2) &
+ (!AB p1:AB->A p2:AB->B AB' p1':AB'->A p2':AB'->B. 
+  (?i:AB->AB' j. i o j = Id(AB') & j o i = Id(AB) &
+   p1' o i = p1 & p2' o i = p2 &
+   p1 o j = p1' & p2 o j = p2')==>
+  (?i:AB'->AB j. i o j = Id(AB) & j o i = Id(AB') &
+   p1 o i = p1' & p2 o i = p2' &
+   p1' o j = p1 & p2' o j = p2)) & 
+ (!AB p1:AB->A p2:AB->B AB' p1':AB'->A p2':AB'->B
+      AB'' p1'':AB''->A p2'':AB''->B. 
+  (?i:AB->AB' j. i o j = Id(AB') & j o i = Id(AB) &
+   p1' o i = p1 & p2' o i = p2 &
+   p1 o j = p1' & p2 o j = p2') &
+  (?i:AB'->AB'' j. i o j = Id(AB'') & j o i = Id(AB') &
+   p1'' o i = p1' & p2'' o i = p2' &
+   p1' o j = p1'' & p2' o j = p2'') ==>
+  (?i:AB->AB'' j. i o j = Id(AB'') & j o i = Id(AB) &
+   p1'' o i = p1 & p2'' o i = p2 &
+   p1 o j = p1'' & p2 o j = p2''))
+ ”)
 
-val p2_def = p1_def |> spec_all 
-                    |> qSKOLEM "p2" [‘A’,‘B’]
-                    |> gen_all 
-                    |> store_as "p2_def";
+local
+val uexth = Pr_uex |> spec_all
+val eth = Pr_ts_ex |> spec_all
+val eqvth = isPair_Reqv
+val fnames = ["*","p1","p2"]
+val arg1 = List.map (dest_var o rastt) 
+                    ["AB","p1:AB->A","p2:AB->B"]
+val arg2 = List.map (dest_var o rastt) 
+                     ["AB'","p1':AB'->A","p2':AB'->B"]
+val eqr = 
+“?i:AB->AB' j. i o j = Id(AB') & j o i = Id(AB) &
+   (p1':AB'->A) o i = p1 & (p2':AB'->B) o i = p2 &
+   p1 o j = p1' & p2 o j = p2'”
+val arg = arg1
+val Q = “isPair(p1:AB->A,p2:AB->B)”
+val argQ = (arg,Q)
+val vl = List.map dest_var [rastt "A",rastt "B"]
+val arg12eqr = (arg1,arg2,eqr)
+val uexth = (Pr_uex |> spec_all)
+in
+val Cross_p12_def = 
+new_spec argQ arg12eqr ["*","p1","p2"] vl eth eqvth (Pr_uex |> spec_all)
+|> gen_all
+end
+
+
+val p2_def = prove_store("p2_def",
+e0
+(rpt strip_tac >> 
+ qspecl_then [‘A’,‘B’] assume_tac Cross_p12_def (* 2 *)
+ >-- (fs[isPair_def] >>
+     first_x_assum (qspecl_then [‘x’,‘y’] (strip_assume_tac o uex_expand)) >>
+     qexists_tac ‘r’ >> arw[]) >>
+ fs[isPair_def] >> 
+ first_x_assum (qspecl_then [‘App(p1(A,B),r)’,‘App(p2(A,B),r)’] assume_tac) >>
+ pop_assum (strip_assume_tac o uex_expand) >>
+ qsuff_tac ‘r = r' & s = r'’ >-- (strip_tac >> arw[]) >>
+ strip_tac >> first_x_assum irule >> arw[])
+(form_goal
+ “∀A B.
+    (∀x y. 
+      ∃r:mem(A*B). App(p1(A,B),r) = x & App(p2(A,B),r) = y) &
+    (∀r s.
+     App(p1(A,B),r) = App(p1(A,B),s) &
+     App(p2(A,B),r) = App(p2(A,B),s) ⇒ r = s)”));
 
 val _ = new_pred "SetPr" [("p1",rel_sort (mk_set "AxB") (mk_set "A")),
                             ("p2",rel_sort (mk_set "AxB") (mk_set "B"))]
@@ -724,12 +670,28 @@ e0
 “!A B. SetPr(p1(A,B),p2(A,B))”)
 
 
-val Pa_def =
+val Pa_def0 =
     Thm_2_8_SetPr |> rewr_rule[SetPr_def]
-                  |> spec_all |> uex_expand
-                  |> qSKOLEM "Pa" [‘f’,‘g’]
-                  |> gen_all
-                  |> store_as "Pa_def";
+                  |> spec_all 
+                  |> qsimple_uex_spec "Pa" [‘f’,‘g’]
+
+val Pa_def = prove_store("Pa_def",
+e0
+(rpt gen_tac >>
+ qspecl_then [‘A’,‘B’] assume_tac Thm_2_8_SetPr >>
+ fs[SetPr_def] >>
+ first_x_assum (qsspecl_then [‘f’,‘g’] (strip_assume_tac o uex_expand)) >>
+ rw[Pa_def0] >> rpt strip_tac >>
+ qsuff_tac ‘fg' = fg & Pa(f,g) = fg’ 
+ >-- (rpt strip_tac >> arw[]) >>
+ strip_tac >> first_x_assum irule >> arw[Pa_def0])
+(form_goal “∀A B X f:X->A g:X->B.
+ (p1(A, B) o Pa(f, g) = f & p2(A, B) o Pa(f, g) = g) &
+ !fg': X -> A * B.
+   p1(A, B) o fg' = f & p2(A, B) o fg' = g ==>
+   fg' = Pa(f, g)”));
+
+
 
 val p12_of_Pa = Pa_def |> spec_all |> conjE1 
                        |> qgen ‘g’ |> qgen ‘B’ |> gen_all
@@ -745,13 +707,8 @@ val p2_of_Pa = p12_of_Pa |> spec_all |> conjE2
 
 val is_Pa = Pa_def |> spec_all |> conjE2 
                    |> qgen ‘g’ |> qgen ‘B’ |> gen_all
-                   |> store_as "p12_of_Pa";
+                   |> store_as "is_Pa";
  
-
-
-val _ = new_pred "SetEz" [("f",rel_sort (mk_set "A") (mk_set "B")),
-                           ("g",rel_sort (mk_set "A") (mk_set "B")),
-                           ("e",rel_sort (mk_set "E") (mk_set "A"))]
 
 (*thesetting is considering two categories at the same time, any thing to do for that?, below is ugly, have not tested if some of e or x0 is a function can be proved rather than stated*)
 
@@ -759,19 +716,6 @@ val SetEz_def =
     qdefine_psym ("SetEz",[‘f:A->B’,‘g:A->B’,‘e:E->A’])
     ‘!X x:X->A.f o x = g o x ==> ?!x0:X->E. x = e o x0’
 
-
-
-val Inj_lcancel = prove_store("Inj_lcancel",
-e0
-(rpt strip_tac >> fs[Inj_def] >>
- rw[GSYM FUN_EXT] >> strip_tac >> 
- qsuff_tac ‘App(m,App(f,a)) = App(m,App(g,a))’ >--
- (strip_tac >> first_x_assum irule >> arw[]) >>
- arw[GSYM App_App_o])
-(form_goal
- “!A B m:A->B.Inj(m) ==>
-  !X f:X->A g:X->A. m o f = m o g ==> f = g”));
- 
 local
 val lemma =
     Thm_2_4|> qspecl [‘A’]
@@ -854,22 +798,172 @@ val AX3 = store_ax("AX3",
 “!A. ?PA e:A~>PA. !S0:1~>A.?!s:mem(PA). !x:mem(A). Holds(S0,dot,x) <=> 
  Holds(e,x,s)”)
 
-
-
 (*
 Theorem 2.12. For any relation R:B↬A, there exists a unique function fR:B→PA such that R(y,x) if and only if ϵ(x,fR(y)). It follows that Set is a topos (and Rel is a power allegory).
 *)
 
-val Pow_def = AX3 |> spec_all
-                  |> qSKOLEM "Pow" [‘A’] 
-                  |> gen_all |> store_as "Pow_def"; 
+val Pow_unique = proved_th $
+e0
+(rpt strip_tac >>
+ qby_tac
+ ‘∀s:mem(PA). ?!s':mem(PA').
+  ∀x. Holds(e,x,s) <=> Holds(e',x,s')’
+ >-- (strip_tac >>
+     strip_assume_tac
+     (AX1_ex |> qspecl [‘1’,‘A’] 
+         |> fVar_sInst_th “P(a:mem(1),b:mem(A))”
+            “Holds(e:A~>PA,b,s)”)  >>
+     first_x_assum (qspecl_then [‘R’] assume_tac) >>
+     first_x_assum (qspecl_then [‘dot’] assume_tac) >> 
+     fs[]) >>
+ drule 
+ (P2fun |> qspecl [‘PA’,‘PA'’] 
+        |> fVar_sInst_th “P(s:mem(PA),s':mem(PA'))”
+           “∀x. Holds(e:A~>PA,x,s) <=> Holds(e':A~>PA',x,s')”) >>
+ pop_assum strip_assume_tac >>
+ qby_tac
+ ‘∀s':mem(PA'). ?!s:mem(PA).
+  ∀x. Holds(e,x,s) <=> Holds(e',x,s')’
+ >-- (strip_tac >>
+     strip_assume_tac
+     (AX1_ex |> qspecl [‘1’,‘A’] 
+         |> fVar_sInst_th “P(a:mem(1),b:mem(A))”
+            “Holds(e':A~>PA',b,s')”)  >>
+     last_x_assum (qspecl_then [‘R’] (assume_tac o GSYM)) >>
+     first_x_assum (qspecl_then [‘dot’] assume_tac) >> 
+     fs[]) >>
+ drule 
+ (P2fun |> qspecl [‘PA'’,‘PA’] 
+        |> fVar_sInst_th “P(s':mem(PA'),s:mem(PA))”
+           “∀x. Holds(e:A~>PA,x,s) <=> Holds(e':A~>PA',x,s')”) >>
+ pop_assum strip_assume_tac >>
+ qexistsl_tac [‘f’,‘f'’] >>  
+ rw[GSYM FUN_EXT,Id_def,App_App_o,GSYM R_EXT,asR_def,GSYM ao_def] >>
+ arw[] >> rpt strip_tac (* 4 *)
+ >-- (first_x_assum (irule o iffLR) >> rw[])
+ >-- (last_x_assum (irule o iffLR) >> rw[]) 
+ >-- (dimp_tac >> rpt strip_tac (* 2 *)
+     >-- (first_x_assum (irule o iffLR) >> arw[]) >>
+     qexists_tac ‘App(f',b)’ >>
+     first_x_assum (qspecl_then [‘b’,‘App(f',b)’] assume_tac) >>
+     fs[]) >>
+ dimp_tac >> rpt strip_tac (* 2 *)
+ >-- (first_x_assum (irule o iffRL) >> arw[]) >>
+ qexists_tac ‘App(f,b)’ >>
+ first_x_assum (qspecl_then [‘b’,‘App(f,b)’] assume_tac) >>
+ fs[])
+(form_goal
+ “∀A PA e:A~> PA PA' e':A~> PA'.
+ (∀S0:1~>A. 
+    ?!s:mem(PA).
+      ∀x. Holds(S0,dot,x) ⇔ Holds(e,x,s)) &
+ (∀S0:1~>A. 
+    ?!s:mem(PA').
+      ∀x. Holds(S0,dot,x) ⇔ Holds(e',x,s)) ⇒
+ ∃i: PA -> PA' j:PA' -> PA.
+  i o j = Id(PA') & j o i = Id(PA) &
+  asR(i) @ e = e' & asR(j) @ e' = e”)
+
+
+val Pow_uex = prove_store("Pow_uex",
+e0
+(qspecl_then [‘A’] strip_assume_tac AX3 >>
+ qexistsl_tac [‘PA’,‘e’] >> arw[] >>
+ rpt strip_tac >> irule Pow_unique >> arw[] )
+(form_goal 
+“?PA e:A~>PA. 
+   (!S0:1~>A.?!s:mem(PA). !x:mem(A). Holds(S0,dot,x) <=> 
+   Holds(e,x,s)) & 
+ ∀PA' e':A~> PA'.
+   (!S0:1~>A.?!s:mem(PA'). !x:mem(A). Holds(S0,dot,x) <=> 
+    Holds(e',x,s)) ⇒
+   ∃i: PA -> PA' j:PA' -> PA.
+  i o j = Id(PA') & j o i = Id(PA) &
+  asR(i) @ e = e' & asR(j) @ e' = e”));
+
+
+val Pow_REFL = proved_th $
+e0
+(rpt strip_tac >> qexistsl_tac [‘Id(PA)’,‘Id(PA)’] >>
+ rw[IdL,IdR,asR_Id,idL])
+(form_goal
+ “∀PA e:A~>PA.
+  ∃i: PA -> PA j:PA -> PA.
+  i o j = Id(PA) & j o i = Id(PA) &
+  asR(i) @ e = e & asR(j) @ e = e”)
+
+
+
+val Pow_SYM = proved_th $
+e0
+(rpt strip_tac >> qexistsl_tac [‘j’,‘i’] >> arw[])
+(form_goal
+ “∀PA e:A~>PA PA' e':A~>PA'.
+  (∃i: PA -> PA' j:PA' -> PA.
+  i o j = Id(PA') & j o i = Id(PA) &
+  asR(i) @ e = e' & asR(j) @ e' = e) ⇒
+  (∃i: PA' -> PA j:PA -> PA'.
+  i o j = Id(PA) & j o i = Id(PA') &
+  asR(i) @ e' = e & asR(j) @ e = e')”)
+
+
+val Pow_SYM = proved_th $
+e0
+(rpt strip_tac >> qexistsl_tac [‘j’,‘i’] >> arw[])
+(form_goal
+ “∀PA e:A~>PA PA' e':A~>PA'.
+  (∃i: PA -> PA' j:PA' -> PA.
+  i o j = Id(PA') & j o i = Id(PA) &
+  asR(i) @ e = e' & asR(j) @ e' = e) ⇒
+  (∃i: PA' -> PA j:PA -> PA'.
+  i o j = Id(PA) & j o i = Id(PA') &
+  asR(i) @ e' = e & asR(j) @ e = e')”)
+
+val Pow_TRANS = proved_th $
+e0
+(rpt strip_tac >>
+ qexistsl_tac [‘i' o i’,‘j o j'’] >> 
+ arw[asR_o,ao_assoc] >>
+ qsuff_tac
+ ‘i' o (i o j) o j' = Id(PA'') & j o (j' o i') o i = Id(PA)’
+ >-- rw[o_assoc] >>
+ arw[IdL,IdR])
+(form_goal
+ “∀PA e:A~>PA PA' e':A~>PA' PA'' e'':A~> PA''.
+  (∃i: PA -> PA' j:PA' -> PA.
+  i o j = Id(PA') & j o i = Id(PA) &
+  asR(i) @ e = e' & asR(j) @ e' = e) &
+  (∃i: PA' -> PA'' j:PA'' -> PA'.
+  i o j = Id(PA'') & j o i = Id(PA') &
+  asR(i) @ e' = e'' & asR(j) @ e'' = e') ⇒ 
+  (∃i: PA -> PA'' j:PA'' -> PA.
+  i o j = Id(PA'') & j o i = Id(PA) &
+  asR(i) @ e = e'' & asR(j) @ e'' = e)”)
+
+local 
+val eth = proved_th $
+e0
+(qspecl_then [‘A’] strip_assume_tac AX3 >>
+ qexistsl_tac [‘PA’,‘e’] >> rw[])
+(form_goal “∃PA e:A~>PA.T”)
+val eqvth = conjI Pow_REFL (conjI Pow_SYM Pow_TRANS) 
+val uexth = Pow_uex
+in
+val Pow_def = 
+    new_spec ([("PA",set_sort),("e",rel_sort (rastt "A") (rastt "PA"))],
+              “!S0:1~>A.?!s:mem(PA). !x:mem(A). Holds(S0,dot,x) <=> 
+                                           Holds(e:A~>PA,x,s)”)
+             ([("PA",set_sort),("e",rel_sort (rastt "A") (rastt "PA"))],
+              [("PA'",set_sort),("e'",rel_sort (rastt "A") (rastt "PA'"))],
+              “∃i: PA -> PA' j:PA' -> PA.
+                 i o j = Id(PA') & j o i = Id(PA) &
+                 asR(i) @ e:A~>PA = e' & asR(j) @ e' = e”)
+             ["Pow","In"] [("A",set_sort)] eth eqvth uexth
+             |> gen_all
+end
+
 
 fun Pow A = mk_fun "Pow" [A]
-
-val In_def = 
-    Pow_def |> spec_all
-            |> qSKOLEM "In" [‘A’] 
-            |> gen_all |> store_as "In_def"; 
 
 (*base change*)
 val BC0_def = 
@@ -877,10 +971,11 @@ val BC0_def =
         |> fVar_sInst_th
            “P(ys:mem(Pow(Y)),zs:mem(Pow(Z)))”
            “!z:mem(Z). Holds(In(Z),z,zs) <=> Holds(In(Y),App(f,z),ys)”
-        |> uex_expand
-        |> qSKOLEM "BC0" [‘f’] |> gen_all
+        |> qsimple_uex_spec "BC0" [‘f’]
+        |> gen_all
         |> store_as "BC0_def";
 
+val In_def = Pow_def 
 
 local 
 val lemma = 
@@ -981,7 +1076,10 @@ fVar_Inst_th
 ("P",([("zs",mem_sort (Pow (mk_set "Z"))),("ys",mem_sort (Pow (mk_set "Y")))],
 “!y:mem(Y). Holds(In(Y),y,ys) <=> ?z:mem(Z).Holds(In(Z),z,zs) & App(f,z) = y”))
 (AX1|> qspecl [‘Pow(Z)’,‘Pow(Y)’]) 
-|> uex_expand |> qSKOLEM "Ex0" [‘f’] |> gen_all
+|> qsimple_uex_spec "Ex0" [‘f’] |> gen_all
+
+(*
+|> uex_expand |> qSKOLEM "Ex0" [‘f’] |> gen_all*)
 
 
 
@@ -990,7 +1088,9 @@ fVar_Inst_th
 ("P",([("zs",mem_sort (Pow (mk_set "Z"))),("ys",mem_sort (Pow (mk_set "Y")))],
 “!y:mem(Y). Holds(In(Y),y,ys) <=> !z:mem(Z). App(f,z) = y ==> Holds(In(Z),z,zs) ”))
 (AX1|> qspecl [‘Pow(Z)’,‘Pow(Y)’]) 
-|> uex_expand |> qSKOLEM "All0" [‘f’] |> gen_all
+|> qsimple_uex_spec "All0" [‘f’] |> gen_all
+
+(*|> uex_expand |> qSKOLEM "All0" [‘f’] |> gen_all *)
 
 
 local
@@ -1039,9 +1139,6 @@ end
 
 
 (*poset order of P(A)*)
-val _ = new_pred "PO" [("S1",mem_sort (Pow (mk_set "A"))),
-                       ("S2",mem_sort (Pow (mk_set "A")))]
-
 val PO_def = qdefine_psym ("PO",[‘S1:mem(Pow(A))’,
                                  ‘S2:mem(Pow(A))’])
 ‘!a. Holds(In(A),a,S1) ==> Holds(In(A),a,S2)’ 
@@ -1050,16 +1147,21 @@ val PO_def = qdefine_psym ("PO",[‘S1:mem(Pow(A))’,
 
 val BC_def = rel2fun |> qsspecl [‘BC0(f:Z->Y)’]
                      |> C mp (BC0_isFun|>qsspecl [‘f:Z->Y’])
+                     |> qsimple_uex_spec "BC" [‘f’]
+                     |> gen_all
+
+(*
                      |> uex2ex_rule 
                      |> qSKOLEM "BC" [‘f’] 
                      |> gen_all
                      |> store_as "BC_def";
+*)
 
 val In_App_BC = prove_store("In_App_BC",
 e0
 (rpt strip_tac >> 
  qspecl_then [‘Y’,‘Z’,‘f’] assume_tac BC_def >>
- qspecl_then [‘Y’,‘Z’,‘f’] (assume_tac o conjE1) BC0_def >>
+ qspecl_then [‘Y’,‘Z’,‘f’] assume_tac BC0_def >>
  dimp_tac >> strip_tac (* 2 *)
  >-- (first_x_assum $ irule o iffLR o iffLR >>
      qexists_tac ‘App(BC(f),ys)’ >> arw[] >>
@@ -1074,16 +1176,20 @@ e0
 
 val Ex_def = rel2fun |> qsspecl [‘Ex0(f:Z->Y)’]
                      |> C mp (Ex0_isFun|>qsspecl [‘f:Z->Y’])
+                     |> qsimple_uex_spec "Ex" [‘f’]
+                     |> gen_all
+
+(*
                      |> uex2ex_rule 
                      |> qSKOLEM "Ex" [‘f’] 
                      |> gen_all
                      |> store_as "Ex_def";
-
+*)
 
 val In_App_Ex = prove_store("In_App_Ex",
 e0
 (rpt strip_tac >> 
- qspecl_then [‘Y’,‘Z’,‘f’] (assume_tac o conjE1) Ex0_def >> 
+ qspecl_then [‘Y’,‘Z’,‘f’] assume_tac Ex0_def >> 
  qspecl_then [‘Y’,‘Z’,‘f’] assume_tac Ex_def >>
  dimp_tac >> strip_tac (* 2 *) >--
  (first_x_assum $ irule o iffLR o iffLR >> 
@@ -1101,15 +1207,20 @@ e0
 
 val All_def = rel2fun |> qsspecl [‘All0(f:Z->Y)’]
                      |> C mp (All0_isFun|>qsspecl [‘f:Z->Y’])
+                     |> qsimple_uex_spec "All" [‘f’]
+                     |> gen_all
+
+(*
                      |> uex2ex_rule 
                      |> qSKOLEM "All" [‘f’] 
                      |> gen_all
                      |> store_as "All_def";
+*)
  
 val In_App_All = prove_store("In_App_All",
 e0
 (rpt strip_tac >> 
- qspecl_then [‘Y’,‘Z’,‘f’] (assume_tac o conjE1) All0_def >> 
+ qspecl_then [‘Y’,‘Z’,‘f’] assume_tac  All0_def >> 
  qspecl_then [‘Y’,‘Z’,‘f’] assume_tac All_def >> 
  dimp_tac >> strip_tac (* 2 *) >--
  (rpt strip_tac >> 
@@ -1126,8 +1237,6 @@ e0
 
 
 
-
- 
 val Thm_2_11_SEx_ex = prove_store("Thm_2_11_SEx_ex",
 e0
 (rpt strip_tac >> rw[PO_def] >> 
@@ -1160,18 +1269,6 @@ e0
   !ys:mem(Pow(Y)) zs:mem(Pow(Z)). PO(App(BC(f),ys),zs) <=> PO(ys,App(All(f),zs))”)); 
 
 
-
-
-val op_DISTR = prove_store("op_DISTR",
-e0
-(rpt strip_tac >> 
- rw[GSYM R_EXT,op_def,GSYM ao_def] >>
- rpt strip_tac >> dimp_tac >> strip_tac (*2 *) >--
- (qexists_tac ‘b'’ >> arw[]) >>
- qexists_tac ‘b'’ >> arw[])
-(form_goal
-“!A B phi:A~>B C psi:B~>C. op(psi @ phi) = op(phi) @ op(psi)”));
-
 (*
 If x and y are elements of a poset, then their meet is an element x∧y of the poset such that:
 
@@ -1183,28 +1280,15 @@ if a≤x and a≤y, then a≤x∧y.
 val Sub_def = qdefine_psym ("Sub",[‘R1:A~>B’,‘R2:A~>B’])
               ‘!a b. Holds(R1,a,b) ==> Holds(R2,a,b)’
               |> gen_all |> store_as "Sub_def";
-
-local 
-val lemma = 
-fVar_Inst_th
-("P",([("a",mem_sort (mk_set "A")),
-        ("b",mem_sort (mk_set "B"))],
-“Holds(R1:A~>B,a,b) & Holds(R2:A~>B,a,b)”))
-(AX1 |> qspecl [‘A’,‘B’]) |> uex_expand
-in
-val Meet_ex = prove_store("Meet_ex",
-e0
-(rpt strip_tac >> strip_assume_tac lemma >> 
- qexists_tac ‘R’ >> arw[] >> rpt strip_tac >> rw[])
-(form_goal 
- “!A B R1:A~>B R2:A~>B. ?M:A~>B. !a b. Holds(M,a,b) <=> Holds(R1,a,b) & Holds(R2,a,b)”));
-end
-
-
-val Meet_def = Meet_ex |> spec_all
-                       |> qSKOLEM "Meet" [‘R1’,‘R2’] 
-                       |> gen_all 
-                       |> store_as "Meet_def"; 
+ 
+val Meet_def = 
+    fVar_Inst_th
+        ("P",([("a",mem_sort (mk_set "A")),
+               ("b",mem_sort (mk_set "B"))],
+              “Holds(R1:A~>B,a,b) & Holds(R2:A~>B,a,b)”))
+        (AX1 |> qspecl [‘A’,‘B’])
+        |> qsimple_uex_spec "Meet" [‘R1’,‘R2’]
+        |> gen_all
 
 val Sub_Meet = prove_store("Sub_Meet",
 e0
@@ -1214,26 +1298,15 @@ e0
 “!A B R1:A~>B R2:A~>B. Sub(Meet(R1,R2),R1) & Sub(Meet(R1,R2),R2) &
  !R0. Sub(R0,R1) & Sub(R0,R2) ==> Sub(R0,Meet(R1,R2))”)); 
 
-local 
-val lemma = 
-fVar_Inst_th
-("P",([("a",mem_sort (mk_set "A")),
-        ("b",mem_sort (mk_set "B"))],
-“Holds(R1:A~>B,a,b) | Holds(R2:A~>B,a,b)”))
-(AX1 |> qspecl [‘A’,‘B’]) |> uex_expand
-in
-val Join_ex = prove_store("Join_ex",
-e0
-(rpt strip_tac >> strip_assume_tac lemma >> 
- qexists_tac ‘R’ >> arw[] >> rpt strip_tac >> rw[])
-(form_goal 
- “!A B R1:A~>B R2:A~>B. ?J:A~>B. !a b. Holds(J,a,b) <=> Holds(R1,a,b) | Holds(R2,a,b)”));
-end
    
-
-val Join_def = Join_ex |> spec_all 
-                       |> qSKOLEM "Join" [‘R1’,‘R2’] 
-                       |> gen_all |> store_as "Join_def";
+val Join_def = 
+    fVar_Inst_th
+        ("P",([("a",mem_sort (mk_set "A")),
+               ("b",mem_sort (mk_set "B"))],
+              “Holds(R1:A~>B,a,b) | Holds(R2:A~>B,a,b)”))
+        (AX1 |> qspecl [‘A’,‘B’]) 
+        |> qsimple_uex_spec "Join" [‘R1’,‘R2’]
+        |> gen_all
 
 (*
 If x and y are elements of a poset P, then their join (or supremum, abbreviate sup, or least upper bound, abbreviated lub), is an element x∨y of the poset such that:
@@ -1390,10 +1463,8 @@ end
 
 (*mem as fun*)
 val MF_def = Thm_2_3_5_el |> spec_all 
-                          |> uex2ex_rule
-                          |> qSKOLEM "MF" [‘a’] 
+                          |> qsimple_uex_spec "MF" [‘a’]
                           |> gen_all
-                          |> store_as "MF_def";
  
 
 (*
@@ -1402,9 +1473,30 @@ Theorem 2.13. For any two sets A and B, there exists a set BA and a function ev:
 Proof. We take BA to be a tabulation of the subset of P(A×B) containing only the functions. More precisely, define F⊆P(A×B) such that s∈F iff for every x∈A, there exists a unique y∈B such that ϵ((x,y),s), and let BA=|F|.  ▮
 *)
 
-val Pair_def = p2_def |> spec_all |> conjE1 |> spec_all 
+val Pair_uex = prove_store("Pair_uex",
+e0
+(rpt strip_tac >>
+ qspecl_then [‘A’,‘B’] strip_assume_tac p2_def >>
+ uex_tac >>
+ first_x_assum (qspecl_then [‘x’,‘y’] strip_assume_tac) >>
+ qexists_tac ‘r’ >> arw[] >>
+ rpt strip_tac >>
+ first_x_assum irule>> arw[])
+(form_goal
+ “∀A B.
+    ∀x y. 
+      ?!r:mem(A*B). App(p1(A,B),r) = x & App(p2(A,B),r) = y”));
+
+val Pair_def = Pair_uex |> spec_all 
+                        |> qsimple_uex_spec "Pair" [‘x’,‘y’]
+                        |> gen_all
+
+(*
+
+p2_def |> spec_all |> conjE1 |> spec_all 
                      |> qSKOLEM "Pair" [‘x’,‘y’] 
                      |> gen_all |> store_as "Pair_def";
+*)
 
 val Pair_App_eq = p2_def |> spec_all |> conjE2 |> gen_all |> store_as "Pair_App_eq";
 
@@ -1434,6 +1526,224 @@ e0
  first_x_assum irule >> rw[Pair_def])
 (form_goal
  “!A B ab:mem(A * B). Pair(App(p1(A,B),ab),App(p2(A,B),ab)) = ab”)); 
+
+
+
+local
+val l = P2fun_uex |> qspecl [‘A’,‘B’] 
+               |> fVar_sInst_th “P(a:mem(A),b:mem(B))”
+                  “App(f:A * X->B,Pair(a,x)) = b”
+in
+val Ap1_uex = prove_store("curry_lemma",
+e0
+(rpt strip_tac >> flip_tac >> irule l >> strip_tac >>
+ uex_tac >> qexists_tac ‘App(f, Pair(x', x))’ >> rw[] >>
+ rpt strip_tac >> arw[]) 
+(form_goal
+ “!A X B f:A * X->B. 
+  !x. ?!fx:A->B. 
+  !a. App(fx,a) = App(f,Pair(a,x))”));
+end
+
+val Ap1_def = 
+    Ap1_uex |> spec_all |> qsimple_uex_spec "Ap1" [‘f’,‘x’]
+            |> qgen ‘f’ |> qgen ‘B’
+            |> gen_all
+            |> store_as "Ap1_def";
+
+
+val Cross_eq = 
+    p2_def |> spec_all |> conjE2 |> gen_all|> store_as "Cross_eq";
+
+
+val App_Pa = prove_store("App_Pa",
+e0
+(rpt strip_tac >>  assume_tac Pa_def >> irule Cross_eq >> rw[Pair_def] >> 
+ arw[GSYM App_App_o])
+(form_goal
+ “!A C f:A->C B D g:B->D. 
+  !ab:mem(A * B).App(Pa(f o p1(A,B),g o p2(A,B)),ab) = Pair(App(f o p1(A,B),ab),App(g o p2(A,B),ab))”));
+
+
+val App_o_p2 = prove_store("App_o_p2",
+e0
+(rw[App_App_o,Pair_def])
+(form_goal
+ “!B C f:B->C.  !A a b.App(f o p2(A,B),Pair(a,b)) = App(f,b)”));
+
+
+val App_o_p1 = prove_store("App_o_p1",
+e0
+(rw[App_App_o,Pair_def])
+(form_goal
+ “!A C f:A->C. !B a b.App(f o p1(A,B),Pair(a,b)) = App(f,a)”));
+
+
+val Fst_def = qdefine_fsym("Fst",[‘x:mem(A*B)’]) ‘App(p1(A,B),x)’
+                          |> GSYM
+
+val Snd_def = qdefine_fsym("Snd",[‘x:mem(A*B)’]) ‘App(p2(A,B),x)’
+                          |> GSYM
+
+
+val Pair_def' = Pair_def |> rewr_rule[Fst_def,Snd_def]|> gen_all
+                         |> store_as "Pair_def'";
+
+val Pair_Fst_Snd = Pair_component |> rewr_rule[Fst_def,Snd_def] |> store_as "Pair_Fst_Snd";
+
+
+
+
+val Pair_has_comp = prove_store("Pair_has_comp",
+e0
+(rpt strip_tac >> 
+ qexistsl_tac [‘Fst(ab)’,‘Snd(ab)’]>>
+ rw[Pair_Fst_Snd])
+(form_goal
+ “!A B ab:mem(A * B). ?a b. ab = Pair(a,b)”));
+
+val p12_of_Pair = Pair_def |> store_as "p12_of_Pair";  
+
+
+
+fun dest_cross t = 
+    case view_term t of 
+        vFun("*",_,[A,B])=> (A,B)
+      | _ => raise simple_fail "dest_cross.not a cross";
+               
+
+fun mk_Pair a b = mk_fun "Pair" [a,b]
+
+fun forall_cross_fconv f = 
+    let val (pv as (n,s),b) = dest_forall f 
+        val pset = s |> dest_sort |> #2  |> hd
+        val (A,B) = dest_cross pset 
+        val pt = mk_var pv
+        val eth = Pair_has_comp |> specl [A,B,pt]
+        val (ocv1 as (ocn1,ocs1),ob1) = dest_exists (concl eth) 
+        val (ocv2 as (ocn2,ocs2),ob2) = dest_exists ob1
+        val avoids = fvf b
+        val ct1 = pvariantt avoids (mk_var ocv1)
+        val ct2 = pvariantt avoids (mk_var ocv2)
+        val (cv1 as (cn1,cs1)) = dest_var ct1
+        val (cv2 as (cn2,cs2)) = dest_var ct2
+        val b1 = substf (ocv1,ct1) ob1
+        val b2 = substf (ocv2,ct2) (substf (ocv1,ct1) ob2)
+        val pair = mk_Pair ct1 ct2 
+        val b' = substf (pv,pair) b
+        val new = mk_forall cn1 cs1 (mk_forall cn2 cs2 b')
+        val l2r = f |> assume |> allE pair 
+                    |> simple_genl [cv1,cv2]
+                    |> disch f
+        val eth1 = b1 |> assume 
+        val r2l = new |> assume |> specl [ct1,ct2]
+                      |> rewr_rule[GSYM $ assume b2]
+                      |> existsE cv2 eth1 
+                      |> existsE cv1 eth
+                      |> allI pv
+                      |> disch new
+    in dimpI l2r r2l 
+    end
+
+
+
+fun basic_fconv_tac c fc = fconv_tac $ basic_fconv c fc;
+
+fun depth_fconv_tac c fc = fconv_tac $ depth_fconv c fc;
+
+val forall_cross_tac =  depth_fconv_tac no_conv forall_cross_fconv;
+
+
+
+val App_Pa_distr = prove_store("App_Pa_distr",
+e0
+(rpt strip_tac >> 
+ qsspecl_then [‘ App(Pa(f, g), x)’] (assume_tac o GSYM) Pair_component >> 
+ once_arw[] >> rw[Pair_eq_eq,GSYM App_App_o,p12_of_Pa])
+(form_goal
+“!X A f:X->A B g:X->B x. App(Pa(f:X->A,g:X->B),x) = Pair(App(f,x),App(g,x))”));
+
+val App_Pa_Pair = App_Pa_distr |> store_as "App_Pa_Pair";
+
+
+(*Parallel product arrow*)
+val Prla_def = 
+    qdefine_fsym ("Prla",[‘f:A->B’,‘g:C->D’])
+    ‘Pa(f o p1(A,C),g o p2(A,C))’
+    |> gen_all |> store_as "Prla_def";
+
+val App_Prla = prove_store("App_Prla",
+e0
+(rpt strip_tac >> rw[Prla_def,App_Pa_Pair] >>
+ rw[App_App_o,p12_of_Pair] )
+(form_goal “!A B f:A->B X Y g:X->Y a x.App(Prla(f,g),Pair(a,x)) = 
+Pair(App(f,a),App(g,x))”));
+
+
+val Exp_ev_unique = prove_store("Exp_ev_unique",
+e0
+(rpt strip_tac >> 
+ qby_tac
+ ‘∀a2b.?!a2b'.∀a. App(Ap1(ev,a2b),a) = App(ev',Pair(a,a2b'))’
+ >-- (strip_tac >>
+     first_x_assum (qsspecl_then [‘Ap1(ev,a2b)’] assume_tac) >>
+     flip_tac >> arw[]) >>
+ drule 
+ (P2fun |> qspecl [‘A2B’,‘A2B'’] 
+        |> fVar_sInst_th “P(a2b:mem(A2B),a2b':mem(A2B'))”
+           “∀a. App(Ap1(ev:A * A2B -> B,a2b),a) = 
+                App(ev':A * A2B' -> B,Pair(a,a2b'))”) >>
+ pop_assum (x_choose_then "i" assume_tac) >>
+ qby_tac
+ ‘∀a2b'.?!a2b.∀a. App(Ap1(ev',a2b'),a) = App(ev,Pair(a,a2b))’
+ >-- (strip_tac >>
+     first_x_assum (qsspecl_then [‘Ap1(ev',a2b')’] assume_tac) >>
+     flip_tac >> arw[]) >>
+ drule 
+ (P2fun |> qspecl [‘A2B'’,‘A2B’] 
+        |> fVar_sInst_th “P(a2b':mem(A2B'),a2b:mem(A2B))”
+           “∀a. App(Ap1(ev':A * A2B' -> B,a2b'),a) = 
+                App(ev:A * A2B -> B,Pair(a,a2b))”) >>
+ pop_assum (x_choose_then "j" assume_tac) >>
+ qexistsl_tac [‘i’,‘j’] >> 
+ qby_tac
+ ‘i o j = Id(A2B')’ 
+ >-- (rw[GSYM FUN_EXT,Id_def,App_App_o] >> arw[] >>
+     strip_tac >>
+     last_x_assum (qsspecl_then [‘a’,‘App(j,a)’] assume_tac) >>
+     fs[] >> 
+     pop_assum (assume_tac o GSYM) >> arw[Ap1_def]) >>
+ qby_tac
+ ‘j o i = Id(A2B)’ 
+ >-- (rw[GSYM FUN_EXT,Id_def,App_App_o] >> arw[] >>
+     strip_tac >>
+     first_x_assum (qsspecl_then [‘a’,‘App(i,a)’] assume_tac) >>
+     fs[] >> 
+     pop_assum (assume_tac o GSYM) >> arw[Ap1_def]) >>
+ arw[] >>
+ qby_tac
+ ‘ev' o Prla(Id(A), i) = ev’ 
+ >-- (rw[GSYM FUN_EXT] >> forall_cross_tac >> 
+     rw[App_App_o,App_Prla,Id_def] >>
+     fs[Ap1_def] >>
+     flip_tac >> rpt strip_tac >>
+     first_x_assum (irule o iffLR) >> rw[]) >>
+ qby_tac
+ ‘ev o Prla(Id(A), j) = ev'’ 
+ >-- (rw[GSYM FUN_EXT] >> forall_cross_tac >> 
+     rw[App_App_o,App_Prla,Id_def] >>
+     fs[Ap1_def] >>
+     flip_tac >> rpt strip_tac >>
+     first_x_assum (irule o iffLR) >> rw[]) >>
+ arw[])
+(form_goal 
+ “∀A B A2B ev:A * A2B ->B A2B' ev': A * A2B' -> B.
+  (!f:A->B.?!sf:mem(A2B).!a:mem(A).App(ev,Pair(a,sf)) = App(f,a)) &
+  (!f:A->B.?!sf:mem(A2B').!a:mem(A).App(ev',Pair(a,sf)) = App(f,a)) ⇒
+  ∃i: A2B -> A2B' j:A2B' -> A2B. 
+   i o j = Id(A2B') & j o i = Id(A2B) &
+   ev' o Prla(Id(A),i)  = ev & ev o Prla(Id(A),j) = ev'”));
+
 
 local 
 val lemma = 
@@ -1563,56 +1873,166 @@ e0
  !f:A->B.?!sf:mem(A2B).!a:mem(A).App(ev,Pair(a,sf)) = App(f,a)”));
 end
 
-(*equiv principle of exp*)
+
+val Exp_ex_uex = prove_store("Exp_ex_uex",
+e0
+(rpt strip_tac >>
+ qspecl_then [‘A’,‘B’] strip_assume_tac Exp_ex >>
+ qexistsl_tac [‘A2B’,‘ev’] >> arw[] >> 
+ rpt strip_tac >> irule Exp_ev_unique >> arw[])
+(form_goal
+“!A B.
+ ?A2B ev:A * A2B ->B. 
+ (!f:A->B.?!sf:mem(A2B).!a:mem(A).App(ev,Pair(a,sf)) = App(f,a)) &
+ ∀A2B' ev':A * A2B' -> B.
+ (∀f:A->B.?!sf:mem(A2B').!a:mem(A).App(ev',Pair(a,sf)) = App(f,a)) ⇒
+ ∃i: A2B -> A2B' j:A2B' -> A2B. 
+   i o j = Id(A2B') & j o i = Id(A2B) &
+   ev' o Prla(Id(A),i)  = ev & ev o Prla(Id(A),j) = ev'”));
+
+val Prla_Id = prove_store("Prla_Id",
+e0
+(rpt strip_tac >> rw[GSYM FUN_EXT] >> strip_tac >>
+ qsspecl_then [‘a’] strip_assume_tac Pair_has_comp >>
+ arw[App_Prla,Id_def])
+(form_goal “∀A B.Prla(Id(A),Id(B)) = Id(A*B)”));
 
 
-
-
-val Exp_def = Exp_ex |> spec_all |> qSKOLEM "Exp" [‘A’,‘B’]
-                     |> gen_all |> store_as "Exp_def"; 
-
-val Ev_def = Exp_def |> spec_all |> qSKOLEM "Ev" [‘A’,‘B’]
-                     |> gen_all |> store_as "Ev_def";
-
-val Tpm_def = Ev_def |> spec_all |> uex_expand
-                     |> qSKOLEM  "Tpm" [‘f’]
-                     |> disch_all |> gen_all
-                     |> store_as "Tpm_def";  
-
+val Prla_split = prove_store("Prla_split",
+e0
+(rpt strip_tac >> rw[GSYM FUN_EXT] >>
+ strip_tac >>
+ qsspecl_then [‘a’] (x_choosel_then ["a1","b1"] assume_tac) Pair_has_comp >>
+ arw[App_App_o,App_Prla])
+(form_goal “∀A1 A2 f1:A1-> A2 A3 f2:A2->A3 B1 B2 g1:B1->B2 B3 g2:B2->B3.
+ Prla(f2 o f1,g2 o g1) = Prla(f2,g2) o Prla(f1,g1)”));
 
  
+val Prla_lsplit1 = prove_store("Prla_lsplit1",
+e0
+(rpt strip_tac >>
+ qsspecl_then [‘f1’,‘f2’,‘Id(B1)’,‘g’] assume_tac Prla_split >>
+ fs[IdR])
+(form_goal “∀A1 A2 f1:A1-> A2 A3 f2:A2->A3 B1 B2 g:B1->B2.
+ Prla(f2 o f1,g) = Prla(f2,g) o Prla(f1,Id(B1))”));
 
 
-(*apply only first arg*)
+val Prla_lsplit2 = prove_store("Prla_lsplit2",
+e0
+(rpt strip_tac >>
+ qsspecl_then [‘f1’,‘f2’,‘g’,‘Id(B2)’] assume_tac Prla_split >>
+ fs[IdL])
+(form_goal “∀A1 A2 f1:A1-> A2 A3 f2:A2->A3 B1 B2 g:B1->B2.
+ Prla(f2 o f1,g) = Prla(f2,Id(B2)) o Prla(f1,g)”));
+
+val Prla_rsplit2 = 
+Prla_split |> qsspecl [‘f:A1->A2’,‘Id(A2)’,‘g1:B1->B2’,‘g2:B2->B3’] 
+           |> rewr_rule[IdL] |> gen_all
 
 
-(*under test
-example:
-val ivar = dest_var $ rastt "a:mem(A)"
-val otm = rastt "App(f:A * X -> B,Pair(a,x))"
-
-*)
-
- 
+val Prla_rsplit1 = 
+Prla_split |> qsspecl [‘Id(A1)’,‘f:A1->A2’,‘g1:B1->B2’,‘g2:B2->B3’] 
+           |> rewr_rule[IdR] |> gen_all
 
 
+
+val Exp_uex_refl = proved_th $
+e0
+(rpt strip_tac >> qexistsl_tac [‘Id(A2B)’,‘Id(A2B)’] >> 
+ rw[IdL,IdR,Prla_Id])
+(form_goal 
+ “∀A2B ev:A * A2B -> B.
+  ∃i: A2B -> A2B j:A2B -> A2B. 
+   i o j = Id(A2B) & j o i = Id(A2B) &
+   ev o Prla(Id(A),i)  = ev & ev o Prla(Id(A),j) = ev”)
+
+
+val Exp_uex_sym = proved_th $
+e0
+(rpt strip_tac >> qexistsl_tac [‘j’,‘i’] >> arw[])
+(form_goal 
+ “∀A2B ev:A * A2B -> B A2B' ev':A * A2B' -> B.
+  (∃i: A2B -> A2B' j:A2B' -> A2B. 
+   i o j = Id(A2B') & j o i = Id(A2B) &
+   ev' o Prla(Id(A),i)  = ev & ev o Prla(Id(A),j) = ev') ⇒ 
+  (∃i: A2B' -> A2B j:A2B -> A2B'.
+   i o j = Id(A2B) & j o i = Id(A2B') &
+   ev o Prla(Id(A),i) = ev' & ev' o Prla(Id(A),j) = ev)”)
+
+
+val Exp_uex_trans = proved_th $
+e0
+(rpt strip_tac >>
+ qexistsl_tac [‘i' o i’,‘j o j'’] >> 
+ rw[Prla_rsplit2] >> arw[GSYM o_assoc] >>
+ qsuff_tac
+ ‘i' o (i o j) o j' = Id(A2B'') & j o (j' o i') o i = Id(A2B)’
+ >-- rw[o_assoc] >>
+ arw[IdL,IdR])
+(form_goal 
+ “∀A2B ev:A * A2B -> B A2B' ev':A * A2B' -> B A2B'' ev'':A * A2B'' -> B.
+  (∃i: A2B -> A2B' j:A2B' -> A2B. 
+   i o j = Id(A2B') & j o i = Id(A2B) &
+   ev' o Prla(Id(A),i)  = ev & ev o Prla(Id(A),j) = ev') & 
+  (∃i: A2B' -> A2B'' j:A2B'' -> A2B'.
+   i o j = Id(A2B'') & j o i = Id(A2B') &
+   ev'' o Prla(Id(A),i) = ev' & ev' o Prla(Id(A),j) = ev'') ⇒ 
+  (∃i: A2B -> A2B'' j:A2B'' -> A2B.
+   i o j = Id(A2B'') & j o i = Id(A2B) &
+   ev'' o Prla(Id(A),i) = ev & ev o Prla(Id(A),j) = ev'')”)
+
+local
+val Exp_ev_eqv = conjI Exp_uex_refl (conjI Exp_uex_sym Exp_uex_trans) 
+val arg = [("A2B",set_sort),("ev",fun_sort (rastt "A * A2B") (rastt "B"))]
+val Q = “!f:A->B.?!sf:mem(A2B).!a:mem(A).App(ev,Pair(a,sf)) = App(f,a)”
+val argQ = (arg,Q) 
+val arg1 = arg 
+val arg2 = [("A2B'",set_sort),("ev'",fun_sort (rastt "A * A2B'") (rastt "B"))]
+val eqr = “(∃i: A2B -> A2B' j:A2B' -> A2B. 
+   i o j = Id(A2B') & j o i = Id(A2B) &
+   ev' o Prla(Id(A),i)  = ev:A * A2B ->B & ev o Prla(Id(A),j) = ev')”
+val arg12eqr = (arg1,arg2,eqr) 
+val fnames = ["Exp","Ev"]
+val vl = [("A",set_sort),("B",set_sort)] 
+val eth = proved_th $
+e0
+(qspecl_then [‘A’,‘B’] strip_assume_tac Exp_ex >>
+ qexistsl_tac [‘A2B’,‘ev’] >> rw[])
+(form_goal
+“?A2B ev:A * A2B ->B. T”)
+val eqvth = Exp_ev_eqv
+val uexth = Exp_ex_uex
+in
+val Exp_def =  new_spec argQ arg12eqr fnames vl eth eqvth (spec_all uexth)
+                        |> gen_all
+end
+
+val Ev_def = Exp_def;
+
+
+val Tpm_def0 = Ev_def |> spec_all |> qsimple_uex_spec "Tpm" [‘f’] 
+                      |> gen_all
+
+val Tpm_def = prove_store("Tpm_def",
+e0
+(rpt gen_tac >>
+ qspecl_then [‘A’,‘B’,‘f’] assume_tac Tpm_def0 >>
+ arw[] >>
+ qsspecl_then [‘f’] (strip_assume_tac o uex_expand) Ev_def >>
+ rpt strip_tac >>
+ qsuff_tac ‘sf' = sf & Tpm(f) = sf’ 
+ >-- (strip_tac >> arw[]) >>
+ rpt strip_tac >> first_x_assum irule >> arw[])
+(form_goal
+ “∀A B f:A->B.
+   (∀a.App(Ev(A,B),Pair(a,Tpm(f))) = App(f,a)) &
+   ∀sf'.
+   (∀a.App(Ev(A,B),Pair(a,sf')) = App(f,a)) ⇒
+   sf' = Tpm(f)”));
 
 val is_Tpm = Tpm_def |> spec_all |> conjE2 
                      |> gen_all 
                      |> store_as "is_Tpm";
-
-
-
-val Pair_has_comp = prove_store("Pair_has_comp",
-e0
-(rpt strip_tac >> 
- qexistsl_tac [‘Fst(ab)’,‘Snd(ab)’]>>
- rw[Pair_Fst_Snd])
-(form_goal
- “!A B ab:mem(A * B). ?a b. ab = Pair(a,b)”));
-
-
-
 
 local 
 val l = P2fun' |> qspecl [‘X’,‘Exp(A,B)’]
@@ -1659,46 +2079,28 @@ e0
 end
 
 
-val Tp_def = Tp_ex |> spec_all |> uex_expand
-                   |> qSKOLEM "Tp" [‘f’]
-                   |> store_as "Tp_def";
+val Tp_def0 = 
+    Tp_ex |> spec_all 
+          |> qsimple_uex_spec "Tp" [‘f’]
+          |> store_as "Tp_def";
 
+val Tp_def = prove_store("Tp_def",
+e0
+(qsspecl_then [‘f’] (strip_assume_tac o uex_expand) Tp_ex >>
+ rw[Tp_def0] >>
+ rpt strip_tac >>
+ qsuff_tac ‘h' = h & Tp(f) = h’ 
+ >-- (rpt strip_tac >> arw[]) >> strip_tac >>
+ first_x_assum irule >> arw[Tp_def0])
+(form_goal
+ “Ev(A, B) o Pa(p1(A, X), Tp(f) o p2(A, X)) = f &
+  !h':X -> Exp(A,B).
+   Ev(A, B) o Pa(p1(A, X), h' o p2(A, X)) = f ==> h' = Tp(f)”));
 
 
 val is_Tp = Tp_def |> spec_all
                    |> conjE2 |> gen_all
                    |> store_as "is_Tp";
-
-val Refl_def = qdefine_psym ("Refl",[‘R:A~>A’])
-               ‘!a. Holds(R,a,a)’ |> gen_all |> store_as "Refl_def";
-
-val Sym_def =  qdefine_psym ("Sym",[‘R:A~>A’])
-               ‘!a1 a2. Holds(R,a1,a2) ==> Holds(R,a2,a1)’
-               |> gen_all |> store_as "Sym_def";
-
-
-val Trans_def = qdefine_psym ("Trans",[‘R:A~>A’])
-               ‘!a1 a2 a3. Holds(R,a1,a2) & Holds(R,a2,a3) ==> Holds(R,a1,a3)’
-               |> gen_all |> store_as "Trans_def";
-
-val ER_def = qdefine_psym ("ER",[‘R:A~>A’])
-             ‘Refl(R) & Sym(R) & Trans(R)’
-             |> gen_all |> store_as "ER_def";
-
-val Sym_Trans_Rright = prove_store("Sym_Trans_Rright",
-e0
-(rpt strip_tac >> dimp_tac >> strip_tac (* 2 *) >--
- (qby_tac ‘Holds(R,y,x)’ >-- 
-  (fs[Sym_def] >> first_x_assum rev_drule >> arw[]) >>
-  fs[Trans_def] >> first_x_assum irule >>
-  qexists_tac ‘x’ >> arw[]) >>
- fs[Trans_def] >> first_x_assum irule >>
- qexists_tac ‘y’ >> arw[])
-(form_goal
- “!A R:A~>A.Sym(R) & Trans(R)==> !x y. Holds(R,x,y) ==>
-  (!z.Holds(R,x,z) <=> Holds(R,y,z))”));
-
-
 (*
 
 Theorem 2.14. If R is an equivalence relation on A, then there is a surjective function q:A↠B such that R(x,y) holds iff q(x)=q(y).
@@ -1793,17 +2195,22 @@ val IN_def_P = In_def_P |>rewr_rule[GSYM IN_def]
                         |> GSYM
                         |> store_as "IN_def_P";
 
+val _ = new_fun "N0" (set_sort,[]);
+val _ = new_fun "O0" (mem_sort (rastt "N0"),[]);
+val _ = new_fun "S0" (fun_sort (rastt "N0") (rastt "N0"),[])
+
 val AX4 = new_ax
-“?N0 O0:mem(N0) S0:N0->N0.  (!n:mem(N0). ~(App(S0,n) = O0)) & 
+“(!n:mem(N0). ~(App(S0,n) = O0)) & 
  !n m. App(S0,n) = App(S0,m) <=> n = m”
 
-val N0_def = AX4 |> qSKOLEM "N0" [] |> store_as "N0_def";
+val N0_def = AX4 
 
-val O0_def = N0_def |> qSKOLEM "O0" [] |> store_as "O0_def";
+val O0_def = AX4  
 
-val S0_def = O0_def |> qSKOLEM "S0" [] |> store_as "S0_def";
+val S0_def = AX4  
 
 val N0 = mk_fun "N0" []
+
 
 
 
@@ -1822,6 +2229,14 @@ in
 val BIGINTER_ex = prove_store("BIGINTER_ex",
 e0
 (strip_tac >> 
+ qsuff_tac
+ ‘?BI:Pow(Pow(A)) -> Pow(A). 
+  !sss:mem(Pow(Pow(A))) a:mem(A). IN(a,App(BI,sss)) <=>
+  !ss.IN(ss,sss) ==> IN(a,ss)’ 
+ >-- (strip_tac >>
+     uex_tac >> qexists_tac ‘BI’ >> arw[] >>
+     rpt strip_tac >> rw[GSYM FUN_EXT] >>
+     strip_tac >> irule IN_EXT >> arw[]) >> 
  x_choosel_then ["BI"] strip_assume_tac lemma >>
  qby_tac ‘!sss. ?ss. Holds(BI,sss,ss)’ >--
  (strip_tac >> once_arw[] >> 
@@ -1835,12 +2250,12 @@ e0
  first_x_assum $ irule o iffLR >>
  pop_assum (assume_tac o GSYM) >> arw[])
 (form_goal
- “!A. ?BI:Pow(Pow(A)) -> Pow(A). 
+ “!A. ?!BI:Pow(Pow(A)) -> Pow(A). 
   !sss:mem(Pow(Pow(A))) a:mem(A). IN(a,App(BI,sss)) <=>
   !ss.IN(ss,sss) ==> IN(a,ss)”));
 end
 
-val BI_def = BIGINTER_ex |> spec_all |> qSKOLEM "BI" [‘A’]
+val BI_def = BIGINTER_ex |> spec_all |> qsimple_uex_spec "BI" [‘A’]
                          |> gen_all
                          |> store_as "BI_def"; 
 
@@ -1855,8 +2270,10 @@ e0
  “!A sss:mem(Pow(Pow(A))). ?isss.App(BI(A),sss) = isss”))
 
 
-val BIGINTER_def = BIGINTER_ex |> spec_all |> qSKOLEM "BIGINTER" [‘sss’]
-                               |> store_as "BIGINTER_def";
+val BIGINTER_def = 
+qdefine_fsym("BIGINTER",[‘sss:mem(Pow(Pow(A)))’]) 
+‘App(BI(A),sss)’ |> GSYM
+
 
 val IN_BIGINTER = BI_def |> rewr_rule[BIGINTER_def] 
                          |> store_as "IN_BIGINTER";
@@ -1899,52 +2316,165 @@ val inN_cases = inN_cases1 |> store_as "inN_cases";
 val inN_rules = inN_rules3 |> store_as "inN_rules";
 
 
-(*Thm_2_4 is TYPE_DEFINITION, not easy to express it as a thm because the first input is a lambda abs, is this the reason of claiming Thm_2_4 is the best form of TYPE_DEFINITION? *)
 
 
-
-(*lift lemmas not require R to be a full relation, hopefully can also be used for definition of Z or Q, where the relation are between power sets*)
-
-local 
-val l = 
-    P2fun' |> qspecl [‘A’,‘A’]
-           |> fVar_sInst_th “P(x:mem(A),y:mem(A))”
-              “ Holds(R:A0~>A0,App(i:A->A0,x),App(i,y))”
-in
-val Inj_lift_R_lemma = prove_store("Inj_lift_R_lemma",
+val Inj_ex_uex = prove_store("Inj_ex_uex",
 e0
-(rpt strip_tac >> rw[App_App_o] >> irule l >> arw[]
- )
-(form_goal “!A A0 i:A->A0. Inj(i) ==>
- !R:A0~>A0. (!a1:mem(A). ?!a2:mem(A). Holds(R,App(i,a1),App(i,a2))) ==>
- ?f:A->A. (!a. Holds(R,App(i,a),App(i o f,a)))”));
-end
+(rpt strip_tac >> dimp_tac >> strip_tac (* 2 *)
+ >-- first_x_assum (accept_tac o uex2ex_rule) >>
+ uex_tac >> qexists_tac ‘a’ >> arw[] >> rpt strip_tac >>
+ fs[Inj_def] >> first_x_assum irule >> arw[])
+(form_goal “!A B f:A->B. Inj(f) ==>
+ !b. (?!a.App(f,a) = b) <=> (?a.App(f,a) = b)”));
 
-val asR_def = asR_def |> gen_all
-
-val Inj_lift_fun_lemma = prove_store("Inj_lift_fun_lemma",
+val Thm_2_4_unique = proved_th $
 e0
 (rpt strip_tac >>
- drule Inj_lift_R_lemma >>
- first_x_assum (qspecl_then [‘asR(f0)’] assume_tac) >>
- qsuff_tac ‘?f:A->A.!a. Holds(asR(f0), App(i, a), App(i o f, a))’ 
- >-- (strip_tac >> qexists_tac ‘f’ >> 
-     qspecl_then [‘A0’,‘A0’,‘f0’] assume_tac asR_def >>
-     fs[App_App_o]) >>
- first_x_assum irule >> strip_tac >> uex_tac >>
- first_x_assum (qspecl_then [‘a1’] strip_assume_tac) >> 
- qexists_tac ‘a2’ >> 
- qspecl_then [‘A0’,‘A0’,‘f0’] assume_tac asR_def >> arw[] >>
- fs[App_App_o] >> rpt strip_tac >> fs[Inj_def] >>
- first_x_assum drule >> arw[])
-(form_goal “!A A0 i:A->A0. Inj(i) ==>
- !f0:A0->A0. (!a1:mem(A). ?a2:mem(A). App(f0 o i,a1) = App(i,a2)) ==>
- ?f:A->A. (!a. App(i o f,a) = App(f0 o i,a))”));
+ qby_tac
+ ‘∀b. ?!b'. App(i,b) = App(i',b')’ 
+ >-- (strip_tac >> flip_tac >> irule $ iffRL Inj_ex_uex >>
+     arw[] >> flip_tac >> pop_assum (assume_tac o GSYM) >> arw[] >>
+     qexists_tac ‘b’ >> rw[]) >>
+ drule (P2fun |> qspecl [‘B’,‘B'’] 
+              |> fVar_sInst_th “P(b:mem(B),b':mem(B'))”
+                 “App(i:B->A,b) = App(i':B'->A,b')”) >>
+ pop_assum strip_assume_tac >>
+ qby_tac
+ ‘∀b'. ?!b. App(i,b) = App(i',b')’ 
+ >-- (strip_tac >>  irule $ iffRL Inj_ex_uex >>
+     arw[] >> flip_tac >> 
+     last_x_assum (K all_tac) >>
+     last_x_assum (assume_tac o GSYM) >> arw[] >>
+     qexists_tac ‘b'’ >> rw[]) >>
+ drule (P2fun |> qspecl [‘B'’,‘B’] 
+              |> fVar_sInst_th “P(b':mem(B'),b:mem(B))”
+                 “App(i:B->A,b) = App(i':B'->A,b')”) >>
+ pop_assum strip_assume_tac >> 
+ qexistsl_tac [‘f’,‘f'’] >> rw[GSYM FUN_EXT,App_App_o,Id_def] >>
+ arw[] >>
+ qsuff_tac
+ ‘(!a. App(i, App(f', a)) = App(i', a)) &
+  (!a. App(i, a) = App(i', App(f, a)))’ 
+ >-- (rpt strip_tac >> arw[]) >>
+ pop_assum (assume_tac o GSYM) >> arw[] >>
+ pop_assum (assume_tac o GSYM) >> arw[] >>
+ qpick_x_assum
+ ‘∀a b. App(f,a) = b ⇔ App(i,a) = App(i',b)’ (assume_tac o GSYM) >>
+ arw[])
+(form_goal “
+ ∀A B i:B->A B' i'.
+ (Inj(i) &
+      (∀a. P(a) <=> ∃b:mem(B). a = App(i,b))) & 
+ (Inj(i') & 
+      (∀a. P(a) ⇔ ∃b:mem(B'). a = App(i',b))) ⇒
+  ∃f:B -> B' g:B' -> B. 
+     f o g = Id(B') &
+     g o f = Id(B) &
+     i' o f = i & i o g = i'”)
 
-val N_def = Thm_2_4 |> qspecl [‘N0’] 
-                    |> fVar_sInst_th 
-                       “P(a:mem(N0))” “IN(a,inNs)”
-                    |> qSKOLEM "N" [] |> qSKOLEM "iN" []
+
+val Thm_2_4' = proved_th $
+e0
+(strip_tac >>
+ qspecl_then [‘A’] strip_assume_tac Thm_2_4 >> 
+  qexistsl_tac [‘B’,‘i’] >> arw[] >>
+ rpt strip_tac >>
+ irule Thm_2_4_unique >> arw[])
+(form_goal 
+ “∀A. 
+    ∃B i:B->A. 
+     (Inj(i) &
+      (∀a. P(a) <=> ∃b:mem(B). a = App(i,b))) &
+     (∀B' i':B'->A.
+      Inj(i') & 
+      (∀a. P(a) ⇔ ∃b:mem(B'). a = App(i',b)) ⇒
+     ∃f:B -> B' g:B' -> B. 
+     f o g = Id(B') &
+     g o f = Id(B) &
+     i' o f = i & i o g = i')”)
+
+
+
+val T24_ts_ex = proved_th $
+e0
+(strip_tac >> qexistsl_tac [‘A’,‘Id(A)’] >> rw[])
+(form_goal “!A. ?B i:B->A. T”)
+
+val Rrefl = proved_th $
+e0
+(rpt strip_tac >> qexistsl_tac [‘Id(B)’,‘Id(B)’] >> rw[IdR,IdL])
+(form_goal 
+ “∀B i:B->A. 
+  ∃f:B ->B g:B->B. f o g = Id(B) & g o f = Id(B) &
+    i o f = i & i o g = i”)
+
+val Rsym = proved_th $
+e0
+(rpt strip_tac >> qexistsl_tac [‘g’,‘f’] >> arw[])
+(form_goal 
+“∀B i:B ->A B' i':B' -> A. 
+ (∃f:B->B' g:B'->B.
+  f o g = Id(B') & g o f = Id(B) &
+  i' o f = i & i o g = i') ⇒ 
+ (∃f:B'->B g:B->B'.
+  f o g = Id(B) & g o f = Id(B') &
+  i o f = i' & i' o g = i)”)
+
+
+val Rtrans = proved_th $
+e0
+(rpt strip_tac >> qexistsl_tac [‘f' o f’,‘g o g'’] >> arw[] >>
+ arw[GSYM o_assoc] >> 
+ qsuff_tac
+ ‘f' o (f o g) o g' = Id(B'') & g o (g' o f') o f = Id(B)’ 
+ >-- rw[o_assoc] >>
+ arw[IdL,IdR])
+(form_goal 
+“∀B i:B ->A B' i':B' -> A B'' i'':B''->A. 
+ (∃f:B->B' g:B'->B.
+  f o g = Id(B') & g o f = Id(B) &
+  i' o f = i & i o g = i') & 
+ (∃f:B'->B'' g:B''->B'.
+  f o g = Id(B'') & g o f = Id(B') &
+  i'' o f = i' & i' o g = i'') ⇒
+ (∃f:B->B'' g:B''->B.
+  f o g = Id(B'') & g o f = Id(B) &
+  i'' o f = i & i o g = i'')”)
+
+val T24_eqv = conjI Rrefl (conjI Rsym Rtrans)
+
+
+val set_spec_eqv = T24_eqv |> gen_all
+
+val set_spec_arg12eqr0 = 
+([("B",set_sort),("i",fun_sort (rastt "B") (rastt "A"))],
+ [("B'",set_sort),("i'",fun_sort (rastt "B'") (rastt "A"))],
+ “(∃f:B->B' g:B'->B.
+           f o g = Id(B') & g o f = Id(B) &
+           i' o f = i & i o g = i':B'->A)”)
+
+
+fun set_spec oriset sname iname fvs uexth = 
+    let val cuexth = concl uexth 
+        val (buexth,arg) = strip_exists cuexth 
+        val (Q,_) = dest_conj buexth
+        val argQ = (arg,Q) 
+        val tenv = mk_tinst [(("A",set_sort),oriset)]
+        val arg12eqr = 
+            (List.map (dest_var o (inst_term (vd_of tenv)) o mk_var) 
+                      (#1 set_spec_arg12eqr0),
+            List.map (dest_var o (inst_term (vd_of tenv)) o mk_var) 
+                      (#2 set_spec_arg12eqr0),
+            inst_form tenv (#3 set_spec_arg12eqr0))
+        val eth = T24_ts_ex |> allE oriset
+        val eqvth = set_spec_eqv |> allE oriset
+    in new_spec argQ arg12eqr [sname,iname] fvs eth eqvth uexth
+    end
+
+val N_def = Thm_2_4' |> qspecl [‘N0’] 
+                     |> fVar_sInst_th 
+                     “P(a:mem(N0))” “IN(a,inNs)”
+                     |> set_spec (rastt "N0") "N" "iN" []
 
 val iN_Inj = N_def |> conjE1 |> store_as "iN_Inj"; 
 
@@ -1965,20 +2495,29 @@ e0
 (form_goal “!n1:mem(N).?n2:mem(N).App(S0 o iN, n1) = App(iN,n2)”));
 
 val SUC_def =
- Inj_lift_fun_lemma |> qsspecl [‘iN’] 
+ Inj_lift_fun_lemma' |> qsspecl [‘iN’] 
                     |> C mp iN_Inj
                     |> qspecl [‘S0’]
                     |> C mp SUC_ex_lemma 
-                    |> qSKOLEM "SUC" [] 
+                    |> qsimple_uex_spec "SUC" []
                     |> store_as "SUC_def";
 
-val O_def = inN_rules |> conjE1 |> rewr_rule[N_def] 
-                      |> qSKOLEM "O" []
-                      |> store_as "O_def";
-
-(*iN_eq_eq auto*)
 val iN_eq_eq = iN_Inj |> rewr_rule[Inj_def]
                       |> store_as "iN_eq_eq";
+
+
+val iN_ex_uex = Inj_ex_uex |> qsspecl [‘iN’] 
+                           |> rewr_rule[iN_Inj]
+                           |> GSYM
+
+val O_def = inN_rules |> conjE1 |> rewr_rule[N_def] 
+                      |> GSYM
+                      |> rewr_rule[iN_ex_uex]
+                      |> qsimple_uex_spec "O" []
+                      |> GSYM
+                      |> store_as "O_def";
+
+
 
 val S0_eq_eq = S0_def |> conjE2 |> iffLR |> store_as "S0_eq_eq";
 
@@ -2005,7 +2544,15 @@ e0
 
 val Image_ex = prove_store("Image_ex",
 e0
-(rpt strip_tac >> irule 
+(rpt strip_tac >> 
+ qsuff_tac
+ ‘?im:Pow(A) -> Pow(B). 
+ !sa b. IN(b,App(im,sa)) <=> ?a. IN(a,sa) & b = App(f,a)’
+ >-- (strip_tac >> uex_tac >> qexists_tac ‘im’ >> arw[] >>
+     rpt strip_tac >>
+     irule $ iffLR FUN_EXT >> strip_tac >>
+     irule IN_EXT >> arw[]) >>
+irule 
  (P2fun' |> qspecl [‘Pow(A)’,‘Pow(B)’]
         |> fVar_sInst_th “P(x:mem(Pow(A)),y:mem(Pow(B)))”
         “!b. IN(b,y) <=> ?a. IN(a,x) & b = App(f:A->B,a)”) >>
@@ -2013,31 +2560,33 @@ e0
  (IN_def_P |> qspecl [‘B’] 
            |> fVar_sInst_th “P(b:mem(B))”
            “?a:mem(A). IN(a,x) & b = App(f:A->B,a)”))
-(form_goal “!A B f:A->B. ?im:Pow(A) -> Pow(B). 
+(form_goal “!A B f:A->B. ?!im:Pow(A) -> Pow(B). 
  !sa b. IN(b,App(im,sa)) <=> ?a. IN(a,sa) & b = App(f,a)”));
 
 
 val Image_def = Image_ex |> spec_all
-                         |> qSKOLEM "Image" [‘f’] 
+                         |> qsimple_uex_spec"Image" [‘f’] 
                          |> gen_all
                          |> store_as "Image_def"; 
 
 
 (*a machinary to convert things like O_xor_SUC into N0 form? maybe this:*)
 
-val IMAGE_def = 
-    IN_def_P_ex |> qspecl [‘B’] |> fVar_sInst_th “P(b:mem(B))”
-                “?a. IN(a,s0) & b = App(f:A->B,a)” 
-                |> GSYM 
-                |> qSKOLEM "IMAGE" [‘f’,‘s0’] 
-                |> gen_all
-                |> store_as "IMAGE_def"; 
+val IMAGE_def0 = 
+qdefine_fsym("IMAGE",[‘f:A->B’,‘s0:mem(Pow(A))’])
+‘App(Image(f),s0)’
+
+
+val IMAGE_def = Image_def |> rewr_rule[GSYM IMAGE_def0]
+                          |> qspecl [‘A’,‘B’,‘f:A->B’,‘s0:mem(Pow(A))’]
+                          |> gen_all
+                          |> store_as "IMAGE_def"; 
 
 val Whole_def = 
-    IN_def_P_ex |> qspecl [‘A’] |> fVar_sInst_th “P(a:mem(A))”
+    IN_def_P |> GSYM |> qspecl [‘A’] |> fVar_sInst_th “P(a:mem(A))”
                 “T” 
                 |> rewr_rule [] 
-                |> qSKOLEM "Whole" [‘A’] 
+                |> qsimple_uex_spec "Whole" [‘A’] 
                 |> gen_all
                 |> store_as "Whole_def"; 
 
@@ -2154,7 +2703,7 @@ val AX5 = store_ax("AX5",
 
 
 
-val Sg_def = P2fun'|> qspecl [‘A’,‘Pow(A)’] 
+val Sg_def = P2fun_uex |> qspecl [‘A’,‘Pow(A)’] 
                    |> fVar_sInst_th “P(a:mem(A),s:mem(Pow(A)))”
                       “!a0. IN(a0,s) <=> a0 = a:mem(A)”
                    |> C mp 
@@ -2162,7 +2711,7 @@ val Sg_def = P2fun'|> qspecl [‘A’,‘Pow(A)’]
                                 |> fVar_sInst_th “P(a0:mem(A))”
                                    “a0 = a:mem(A)”
                                 |> qgen ‘a’)
-                   |> qSKOLEM "Sg" [‘A’] |> gen_all
+                   |> qsimple_uex_spec  "Sg" [‘A’] |> gen_all
                    |> store_as "Sg_def";
 
 val Sing_def = qdefine_fsym ("Sing",[‘a:mem(A)’])
@@ -2172,18 +2721,9 @@ val Sing_def = qdefine_fsym ("Sing",[‘a:mem(A)’])
 
 val Empty_def = IN_def_P |> qspecl [‘X’]
                          |> fVar_sInst_th “P(x:mem(X))” “F”
-                         |> uex2ex_rule
-                         |> qSKOLEM "Empty" [‘X’]
+                         |> qsimple_uex_spec "Empty" [‘X’]
                          |> rewr_rule[]
                          |> gen_all |> store_as "Empty_def";
-
-val Inj_eq_eq = prove_store("Inj_eq_eq",
-e0
-(rpt strip_tac >> fs[Inj_def] >> dimp_tac >>
- rpt strip_tac >> arw[] >>
- first_x_assum irule >> arw[])
-(form_goal “!X Y i:X->Y. Inj(i) ==>
- (!x1 x2. App(i,x1) = App(i,x2) <=> x1 =  x2)”));
 
 
 val Sing_eq_eq = prove_store("Sing_eq_eq",
@@ -2203,34 +2743,27 @@ e0
 
 
 
+val tof_def = proved_th $
+e0
+(rpt strip_tac >> flip_tac >>
+ qsuff_tac ‘?f:A->B. 
+ !a. App(f,a)= App(Ev(A,B),Pair(a,f0))’
+ >-- (strip_tac >> uex_tac >> qexists_tac ‘f’ >> arw[] >>
+     rpt strip_tac >> arw[GSYM FUN_EXT]) >>
+ irule (P2fun' |> qspecl [‘A’,‘B’] 
+ |> fVar_sInst_th “P(x:mem(A),y:mem(B))”
+    “y = App(Ev(A,B),Pair(x,f0:mem(Exp(A,B))))”) >>
+ strip_tac >> uex_tac >> qexists_tac ‘App(Ev(A, B), Pair(x, f0))’ >> rw[])
+(form_goal “!A B f0:mem(Exp(A,B)).
+ ?!f:A->B. 
+ !a. App(Ev(A,B),Pair(a,f0)) = App(f,a)”)
+|> spec_all |> qsimple_uex_spec "tof" [‘f0’]
+
+
 val iscoPr_def = qdefine_psym("iscoPr",[‘i1:A->AB’,‘i2:B->AB’])
 ‘!X f:A->X g:B->X.?!fg:AB->X.fg o i1 = f & fg o i2 = g’
 |> qgenl [‘A’,‘B’,‘AB’,‘i1’,‘i2’]
 |> store_as "iscoPr_def";
-
-
-
-
-val Inj_lift_fun = prove_store("Inj_lift_fun",
-e0
-(rpt strip_tac >>
- irule (P2fun' |> qspecl [‘X’,‘A’] 
-        |> fVar_sInst_th “P(x:mem(X),a:mem(A))”
-           “App(i:A->A0,a) = App(f0:X->A0,x)”
-        |> rewr_rule[GSYM App_App_o]) >>
- flip_tac >> strip_tac >> uex_tac >>
- first_x_assum (qspecl_then [‘x’] strip_assume_tac) >>
- qexists_tac ‘a’ >> arw[] >> fs[Inj_def] >> rpt strip_tac >>
- first_x_assum irule >> arw[]
- )
-(form_goal
- “!A A0 i:A-> A0.
-  Inj(i) ==>
-  !X f0:X->A0.
-  (!x. ?a.App(f0,x) = App(i,a))==>
-  ?f:X->A. 
-  !x. App(i o f,x) = App(f0,x)”));
-
 
 
 (* subset of Pow(A) * Pow(B)*)
@@ -2488,19 +3021,3 @@ e0
  rw[GSYM i1_xor_i2])
 (form_goal “!A B ab.~(?b. ab = App(i2(A,B),b)) <=> ?a. ab = App(i1(A,B),a)”));
 
-
-val tof_def = proved_th $
-e0
-(rpt strip_tac >> flip_tac >>
- qsuff_tac ‘?f:A->B. 
- !a. App(f,a)= App(Ev(A,B),Pair(a,f0))’
- >-- (strip_tac >> uex_tac >> qexists_tac ‘f’ >> arw[] >>
-     rpt strip_tac >> arw[GSYM FUN_EXT]) >>
- irule (P2fun' |> qspecl [‘A’,‘B’] 
- |> fVar_sInst_th “P(x:mem(A),y:mem(B))”
-    “y = App(Ev(A,B),Pair(x,f0:mem(Exp(A,B))))”) >>
- strip_tac >> uex_tac >> qexists_tac ‘App(Ev(A, B), Pair(x, f0))’ >> rw[])
-(form_goal “!A B f0:mem(Exp(A,B)).
- ?!f:A->B. 
- !a. App(Ev(A,B),Pair(a,f0)) = App(f,a)”)
-|> spec_all |> uex2ex_rule |> qSKOLEM "tof" [‘f0’]
