SEARexamplecol.sml
@@ -1,0 +1,86 @@
+(*naive application of collection, give the existence of a set which is larger then any power set.*)
+
+
+
+val AX5 = store_ax("AX5",
+“!A.?B p:B->A Y M:B~>Y.  
+ (!b.P(App(p,b),m2s(rsi(M,b)))) & 
+ !a:mem(A) X. P(a,X) ==> ?b. App(p,b) = a”)
+
+
+
+
+val INJ_def = 
+qdefine_psym("INJ",
+[‘f:A->B’,‘s:mem(Pow(A))’,‘t:mem(Pow(B))’])
+‘(!x. IN(x,s) ==> IN(App(f,x),t)) &
+(!x y. IN(x,s) & IN(y,s) ==> App(f,x) = App(f,y) ==>
+ x = y)’ |> gen_all
+
+
+val SURJ_def = 
+qdefine_psym("SURJ",
+[‘f:A->B’,‘s:mem(Pow(A))’,‘t:mem(Pow(B))’])
+‘(!x. IN(x,s) ==> IN(App(f,x),t)) &
+(!x. IN(x,t) ==> ?y. IN(y,s) & App(f,y) = x)’ |> gen_all
+
+ 
+val BIJ_def = 
+qdefine_psym
+("BIJ",[‘f:A->B’,‘s:mem(Pow(A))’,‘t:mem(Pow(B))’])
+‘INJ(f,s,t) & SURJ(f,s,t)’ |> gen_all
+
+val cardeq_def = 
+qdefine_psym("cardeq",[‘s1:mem(Pow(A))’,‘s2:mem(Pow(B))’])
+‘?f.BIJ(f,s1,s2)’
+
+
+val POW_def = IN_def_P |> qspecl [‘Pow(A)’] 
+                       |> fVar_sInst_th “P(s:mem(Pow(A)))”
+                          “SS(s,s0:mem(Pow(A)))”
+                       |> uex2ex_rule 
+                       |> qSKOLEM "POW" [‘s0’]
+                       |> gen_all
+
+
+val nPow_def = qdefine_psym("nPow",[‘n:mem(N)’,‘A’,‘B’])
+‘?X f:X->N. cardeq(FIB(f,O),Whole(A)) & 
+            cardeq(FIB(f,n),Whole(B)) &
+  (!n0. Lt(n0,n) ==>
+   cardeq(POW(FIB(f,n0)),FIB(f,Suc(n0))))’
+|> gen_all
+
+
+val cardleq_def = 
+qdefine_psym("cardleq",[‘s1:mem(Pow(A))’,‘s2:mem(Pow(B))’])
+‘?f:A->B. INJ(f,s1,s2)’ |> gen_all
+
+val nPow_ex = prove_store("nPow_ex",
+e0
+cheat
+(form_goal “!A n. ?An. nPow(n,A,An)”));
+
+val large_ex = prove_store("large_ex",
+e0
+(rpt strip_tac >>
+ assume_tac
+ (AX5 |> qspecl [‘N’] 
+ |> fVar_sInst_th “P(n:mem(N),An)”
+     “nPow(n,A,An)”) >>
+ pop_assum strip_assume_tac >> qexists_tac ‘Y’ >> 
+ rpt strip_tac >>
+ first_x_assum drule >>
+ pop_assum strip_assume_tac >>
+ first_x_assum (qsspecl_then [‘b’] assume_tac) >> 
+ rw[cardleq_def] >> 
+ 
+
+
+ qsspecl_then [‘n’] assume_tac nPow_ex >>
+ pop_assum strip_assume_tac >> )
+(form_goal 
+ “!A. 
+    ?P. 
+      !n An. nPow(n,A,An) ==> cardleq(Whole(An),Whole(P)) ”));
+
+
