SEARnewspec.sml
@@ -1,0 +1,66 @@
+
+val funeqeqvth = proved_th $
+e0
+(rpt strip_tac >> arw[])
+(form_goal “∀A B. (!i:A->B. i = i) &
+ (!i:A->B i':A->B. i = i' ==> i' = i) &
+ (!i:A->B i':A->B i'':A->B. 
+   i = i' & i' = i'' ==> i = i'')”)
+
+
+val releqeqvth = proved_th $
+e0
+(rpt strip_tac >> arw[])
+(form_goal “∀A B. (!i:A~>B. i = i) &
+ (!i:A~>B i':A~>B. i = i' ==> i' = i) &
+ (!i:A~>B i':A~>B i'':A~>B. 
+   i = i' & i' = i'' ==> i = i'')”)
+
+
+val memeqeqvth = proved_th $
+e0
+(rpt strip_tac >> arw[])
+(form_goal “∀A. (!i:mem(A). i = i) &
+ (!i:mem(A) i':mem(A). i = i' ==> i' = i) &
+ (!i:mem(A) i':mem(A) i'':mem(A). 
+   i = i' & i' = i'' ==> i = i'')”)
+
+
+
+fun uex_spec fname vl eth uexth0 = 
+    let 
+        val ((_,st),_) = dest_uex (concl uexth0)
+        val stn = st |> dest_sort |> #1
+        val dependson = st |> dest_sort |> #2 
+        val eqvth = if stn = "mem" then memeqeqvth |> specl dependson else 
+                    if stn = "fun" then funeqeqvth |> specl dependson else
+                    if stn = "rel" then releqeqvth |> specl dependson else
+                    raise simple_fail "uex_spec.ill-formed sort"
+        val uexth = uex_expand' uexth0
+        val (arg,Q) = dest_uex (concl uexth0)
+        val argQ = ([arg],Q)
+        val arg' = dest_var (pvariantt (fvf Q) (mk_var arg)) 
+        val equality = mk_eq (mk_var arg) (mk_var arg') 
+        val arg12eqr = ([arg],[arg'],equality) 
+    in new_spec argQ arg12eqr [fname] vl eth eqvth uexth
+    end
+
+fun quex_spec fname qvl eth uexth0 = 
+    let val tl = List.map (qparse_term_with_cont (cont uexth0)) qvl 
+        val vl = List.map dest_var tl
+    in uex_spec fname vl eth uexth0
+    end
+
+fun simple_uex_spec fname vl uexth0 = 
+    let val uexth = uex_expand' uexth0
+        val eth0 = ex_P_ex (concl uexth)
+        val eth = mp eth0 uexth
+    in uex_spec fname vl eth uexth0 
+    end
+
+
+fun qsimple_uex_spec fname qvl uexth0 = 
+    let val tl = List.map (qparse_term_with_cont (cont uexth0)) qvl 
+        val vl = List.map dest_var tl
+    in simple_uex_spec fname vl uexth0
+    end
