newspec.sml
@@ -1,77 +1,35 @@
 
+fun mk_foralls vl f = 
+    case vl of [] => f 
+             | h :: t => uncurry mk_forall h (mk_foralls t f)
 
 
-val Pr_uex = prove_store("Pr_uex",
-e0
-cheat
-(form_goal “!A B. ?AB p1:AB->A p2:AB ->B. 
- isPr(p1,p2) &
- (!AB' p1':AB'->A p2'. isPr(p1',p2') ==>
-  ?!i:AB->AB' j. i o j = Id(AB') & j o i = Id(AB) &
-  p1' o i = p1 & p2' o i = p2 &
-  p1 o j = p1' & p2 o j = p2')”));
 
-val Pr_ts_ex = proved_th $
-e0
-cheat
-(form_goal “!A B. ?AB p1:AB->A p2:AB ->B. T”)
+fun mk_tinst l = mk_inst l [] 
 
-val Reqv = proved_th $
-e0
-cheat
-(form_goal 
-“(!AB p1:AB->A p2:AB->B.
- ?!i:AB->AB j. i o j = Id(AB) & j o i = Id(AB) &
-  p1 o i = p1 & p2 o i = p2 &
-  p1 o j = p1 & p2 o j = p2) &
- (!AB p1:AB->A p2:AB->B AB' p1':AB'->A p2':AB'->B. 
-  (?!i:AB->AB' j. i o j = Id(AB') & j o i = Id(AB) &
-   p1' o i = p1 & p2' o i = p2 &
-   p1 o j = p1' & p2 o j = p2')==>
-  (?!i:AB'->AB j. i o j = Id(AB) & j o i = Id(AB') &
-   p1 o i = p1' & p2 o i = p2' &
-   p1' o j = p1 & p2' o j = p2)) & 
- (!AB p1:AB->A p2:AB->B AB' p1':AB'->A p2':AB'->B
-      AB'' p1'':AB''->A p2'':AB''->B. 
-  (?!i:AB->AB' j. i o j = Id(AB') & j o i = Id(AB) &
-   p1' o i = p1 & p2' o i = p2 &
-   p1 o j = p1' & p2 o j = p2') &
-  (?!i:AB'->AB'' j. i o j = Id(AB'') & j o i = Id(AB') &
-   p1'' o i = p1' & p2'' o i = p2' &
-   p1' o j = p1'' & p2' o j = p2'') ==>
-  (?!i:AB->AB'' j. i o j = Id(AB'') & j o i = Id(AB) &
-   p1'' o i = p1 & p2'' o i = p2 &
-   p1 o j = p1'' & p2 o j = p2''))
- ”)
+fun addprims l = 
+            case l of [] => l
+                    | (n,s) :: t =>
+                      let val new = (n^"'",s)
+                      in
+                          new :: 
+                          (List.map 
+                               (dest_var o 
+                                (substt ((n,s),mk_var new)) o mk_var) (addprims t))
+                      end
 
-val uexth = Pr_uex |> spec_all
+fun mk_existss nsl f = 
+    case nsl of 
+        [] => f
+      | (h as (n,s)) :: t =>
+        mk_exists n s (mk_existss t f)
 
-val eth = Pr_ts_ex |> spec_all
-
-val eqvth = Reqv
-
-val fnames = ["*","p1","p2"]
-
-(*val iseqr = “P()”*)
-
-
-val arg1 = List.map (dest_var o rastt) 
-                    ["AB","p1:AB->A","p2:AB->B"]
-
-val arg2 = List.map (dest_var o rastt) 
-                     ["AB'","p1':AB'->A","p2':AB'->B"]
-
-val eqr = 
-“?!i:AB->AB' j. i o j = Id(AB') & j o i = Id(AB) &
-   (p1':AB'->A) o i = p1 & (p2':AB'->B) o i = p2 &
-   p1 o j = p1' & p2 o j = p2'”
-
-
-val arg = arg1
-val Q = “isPr(p1:AB->A,p2:AB->B)”
-
-val vl = List.map dest_var [rastt "A",rastt "B"]
-
+fun dest_n_exists n f = 
+    if n = 0 then ([],f) else 
+    let val (l,b) = dest_n_exists (n-1) f
+        val (ns,b1) = dest_exists b
+    in (l @ [ns],b1)
+    end
 
 fun mk_REFL_condf (arg1:(string * sort) list,
                   arg2:(string * sort) list,eqr) = 
@@ -129,6 +87,28 @@ fun mk_ER_condf argseqr =
         val eqvcls = mk_conj reflcl (mk_conj symcl transcl)
     in eqvcls
     end 
+
+
+fun check_REFL argseqr reflth =
+    let val reflcl = mk_REFL_condf argseqr 
+        val _ = eq_form (reflcl,concl reflth)
+    in ()
+    end
+
+
+fun check_SYM argseqr symth =
+    let val symcl = mk_SYM_condf argseqr 
+        val _ = eq_form (symcl,concl symth)
+    in ()
+    end
+
+
+fun check_TRANS argseqr transth =
+    let val transcl = mk_TRANS_condf argseqr 
+        val _ = eq_form (transcl,concl transth)
+    in ()
+    end
+
 
 fun check_ER argseqr eqvth uexth = 
     let val eqvcls = mk_ER_condf argseqr
@@ -209,7 +189,7 @@ fun mk_newfsym fnames vl uexth =
         val recoverex = mk_existss newspvs main
         val sts = List.map snd newspvs
         val (ct,asm) = (cont uexth,ant uexth)
-        fun itmk fnl vl f = (*List.foldl  *)
+        fun itmk fnl sts vl f = 
             case fnl of 
                 [] => (fnl,f)
               | h :: t =>
@@ -217,9 +197,21 @@ fun mk_newfsym fnames vl uexth =
                     val ft = mk_fun (hd fnl) (List.map mk_var vl)
                     val (ns,b) = dest_exists f
                     val f0 = substf (ns,ft) b
-                in itmk (tl fnl) vl f0
+                    val sts' = List.map (substs (ns,ft)) sts
+                in itmk (tl fnl) (tl sts') vl f0
                 end 
-        val (_,conc) = itmk fnames vl recoverex
+(*
+        fun itmk fnl sts vl f = (*List.foldl  *)
+            case fnl of 
+                [] => (fnl,f)
+              | h :: t =>
+                let val _ = new_fun (hd fnl) (hd sts,vl)
+                    val ft = mk_fun (hd fnl) (List.map mk_var vl)
+                    val (ns,b) = dest_exists f
+                    val f0 = substf (ns,ft) b
+                in itmk (tl fnl) (tl sts) vl f0
+                end *)
+        val (_,conc) = itmk fnames sts vl recoverex
     in
         mk_thm(ct,asm,conc)
     end
@@ -234,52 +226,6 @@ fun new_spec argQ arg12eqr
         val _ = check_inputs vl vs0
     in mk_newfsym fnames vl uexth
     end
-
-
-
-val Id_uex = prove_store("Id_uex",
-e0
-(cheat)
-(form_goal “?i:A ->A. (!a.App(i,a) = a) & 
- !i'. (!a.App(i',a) = a) ==> i = i'”));
-
-val uexth = Id_uex
-
-val eth = proved_th $
-e0
-cheat
-(form_goal “?i:A->A.T”)
-
-val vl = [("A",set_sort)]
-
-(*spec of new fsym if the input is a uex theorem with assumptions*)
-
-val fname = "Id"
-
-val argQ = ([dest_var (rastt "i:A->A")],“!a. App(i:A->A,a) = a”)
-
-val arg12eqr = ([dest_var (rastt "i:A->A")],[dest_var (rastt "i':A->A")],
-                “i = i':A->A”)
-
-val eqvth = proved_th $
-e0
-cheat
-(form_goal “(!i:A->A. i = i) &
- (!i:A->A i':A->A. i = i' ==> i' = i) &
- (!i:A->A i':A->A i'':A->A. 
-   i = i' & i' = i'' ==> i = i'')”)
-
-new_spec argQ arg12eqr [fname] vl eth eqvth uexth
-
-
-
-val Id_uex0 = prove_store("Id_uex0",
-e0
-(cheat)
-(form_goal “?!i:A ->A. (!a.App(i,a) = a)”));
-
-val uexth0 = Id_uex0
-
 
 
 fun impr_fconv fc f = 
@@ -297,26 +243,220 @@ fun uex_def' f =
 
 fun uex_expand' th = dimp_mp_l2r th (uex_def' $ concl th)
 
-fun uex_spec fname vl eth uexth0 = 
-    let val uexth = uex_expand' uexth0
-        val (arg,Q) = dest_uex (concl uexth0)
-        val argQ = ([arg],Q)
-        val arg' = dest_var (pvariantt (fvf Q) (mk_var arg)) 
-        val equality = mk_eq (mk_var arg) (mk_var arg') 
-        val arg12eqr = ([arg],[arg'],equality) 
-    in new_spec argQ arg12eqr [fname] vl eth eqvth uexth
-    end
 
+
+(*
 (*simple case of uex_spec, applies only when the assumption list of uex is empty and hence the derivation of soundness existential theorem is automated*)
 
-fun simple_uex_spec fname vl uexth0 = 
-    let val uexth = uex_expand' uexth0
-        val eth0 = ex_P_ex (concl uexth)
-        val eth = mp eth0 uexth
-    in uex_spec fname vl eth uexth0 
-    end
 
 (*simple_uex_spec "Id" [("A",set_sort)] Id_uex0 *)
+
+val Thm_2_4_unique = proved_th $
+e0
+(cheat)
+(form_goal “
+ ∀A B i:B->A B' i'.
+ (Inj(i) &
+      (∀a. P(a) <=> ∃b:mem(B). a = App(i,b))) & 
+ (Inj(i') & 
+      (∀a. P(a) ⇔ ∃b:mem(B'). a = App(i',b))) ⇒
+  ∃f:B -> B' g:B' -> B. 
+     f o g = Id(B') &
+     g o f = Id(B) &
+     i' o f = i & i o g = i'”)
+
+val Thm_2_4' = proved_th $
+e0
+(strip_tac >>
+ qspecl_then [‘A’] strip_assume_tac Thm_2_4 >> 
+  qexistsl_tac [‘B’,‘i’] >> arw[] >>
+ rpt strip_tac >>
+ irule Thm_2_4_unique >> arw[])
+(form_goal 
+ “∀A. 
+    ∃B i:B->A. 
+     (Inj(i) &
+      (∀a. P(a) <=> ∃b:mem(B). a = App(i,b))) &
+     (∀B' i':B'->A.
+      Inj(i') & 
+      (∀a. P(a) ⇔ ∃b:mem(B'). a = App(i',b)) ⇒
+     ∃f:B -> B' g:B' -> B. 
+     f o g = Id(B') &
+     g o f = Id(B) &
+     i' o f = i & i o g = i')”)
+
+
+
+val T24_ts_ex = proved_th $
+e0
+(strip_tac >> qexistsl_tac [‘A’,‘Id(A)’] >> rw[])
+(form_goal “!A. ?B i:B->A. T”)
+
+val Rrefl = proved_th $
+e0
+(rpt strip_tac >> qexistsl_tac [‘Id(B)’,‘Id(B)’] >> rw[IdR,IdL])
+(form_goal 
+ “∀B i:B->A. 
+  ∃f:B ->B g:B->B. f o g = Id(B) & g o f = Id(B) &
+    i o f = i & i o g = i”)
+
+val Rsym = proved_th $
+e0
+(rpt strip_tac >> qexistsl_tac [‘g’,‘f’] >> arw[])
+(form_goal 
+“∀B i:B ->A B' i':B' -> A. 
+ (∃f:B->B' g:B'->B.
+  f o g = Id(B') & g o f = Id(B) &
+  i' o f = i & i o g = i') ⇒ 
+ (∃f:B'->B g:B->B'.
+  f o g = Id(B) & g o f = Id(B') &
+  i o f = i' & i' o g = i)”)
+
+
+val Rtrans = proved_th $
+e0
+(rpt strip_tac >> qexistsl_tac [‘f' o f’,‘g o g'’] >> arw[] >>
+ arw[GSYM o_assoc] >> 
+ qsuff_tac
+ ‘f' o (f o g) o g' = Id(B'') & g o (g' o f') o f = Id(B)’ 
+ >-- rw[o_assoc] >>
+ arw[IdL,IdR])
+(form_goal 
+“∀B i:B ->A B' i':B' -> A B'' i'':B''->A. 
+ (∃f:B->B' g:B'->B.
+  f o g = Id(B') & g o f = Id(B) &
+  i' o f = i & i o g = i') & 
+ (∃f:B'->B'' g:B''->B'.
+  f o g = Id(B'') & g o f = Id(B') &
+  i'' o f = i' & i' o g = i'') ⇒
+ (∃f:B->B'' g:B''->B.
+  f o g = Id(B'') & g o f = Id(B) &
+  i'' o f = i & i o g = i'')”)
+
+val T24_eqv = conjI Rrefl (conjI Rsym Rtrans)
+
+
+val set_spec_eqv = T24_eqv |> gen_all
+
+val set_spec_arg12eqr0 = 
+([("B",set_sort),("i",fun_sort (rastt "B") (rastt "A"))],
+ [("B'",set_sort),("i'",fun_sort (rastt "B'") (rastt "A"))],
+ “(∃f:B->B' g:B'->B.
+           f o g = Id(B') & g o f = Id(B) &
+           i' o f = i & i o g = i':B'->A)”)
+
+
+fun set_spec oriset sname iname fvs uexth = 
+    let val cuexth = concl uexth 
+        val (buexth,arg) = strip_exists cuexth 
+        val (Q,_) = dest_conj buexth
+        val argQ = (arg,Q) 
+        val tenv = mk_tinst [(("A",set_sort),oriset)]
+        val arg12eqr = 
+            (List.map (dest_var o (inst_term (vd_of tenv)) o mk_var) 
+                      (#1 set_spec_arg12eqr0),
+            List.map (dest_var o (inst_term (vd_of tenv)) o mk_var) 
+                      (#2 set_spec_arg12eqr0),
+            inst_form tenv (#3 set_spec_arg12eqr0))
+        val eth = T24_ts_ex |> allE oriset
+        val eqvth = set_spec_eqv |> allE oriset
+    in new_spec argQ arg12eqr [sname,iname] fvs eth eqvth uexth
+    end
+
+
+(*
+val Reqv = conjI Rrefl (conjI Rsym Rtrans)
+
+val arg = [("B",set_sort),("i",fun_sort (rastt "B") (rastt "A"))]
+
+val Q = “(Inj(i:B->A) &
+         (∀a. P(a) <=> ∃b:mem(B). a = App(i,b)))”
+
+val argQ = (arg,Q)
+
+val arg1 = [("B",set_sort),("i",fun_sort (rastt "B") (rastt "A"))]
+
+val arg2 = [("B'",set_sort),("i'",fun_sort (rastt "B'") (rastt "A"))]
+
+val eqr = “(∃f:B->B' g:B'->B.
+           f o g = Id(B') & g o f = Id(B) &
+           i' o f = i & i o g = i':B'->A)”
+
+val arg12eqr = (arg1,arg2,eqr) 
+
+val fnames = ["sset","inc"]
+
+val vl = [("A",set_sort)] (*will have more things in practice*)
+
+val eth = spec_all T24_ts_ex
+
+val uexth = spec_all Thm_2_4'
+
+val eqvth = Reqv
+
+new_spec argQ arg12eqr fnames vl eth eqvth uexth
+
+
+val N_def = Thm_2_4 |> qspecl [‘N0’] 
+                    |> fVar_sInst_th 
+                       “P(a:mem(N0))” “IN(a,inNs)”
+                    |> qSKOLEM "N" [] |> qSKOLEM "iN" []
+
+val uexth = 
+ Thm_2_4' |> qspecl [‘N0’] 
+                    |> fVar_sInst_th 
+                       “P(a:mem(N0))” “IN(a,inNs)”
+
+val fvs:(string * sort) list = []
+
+val sname = "N"
+
+val iname = "iN"
+
+
+val oriset = rastt "N0"
+
+
+set_spec (rastt "Pow(N * X)") "List" "iL" [("X",set_sort)] 
+
+ (Thm_2_4' |> qspecl [‘Pow(N * X)’] 
+                    |> fVar_sInst_th 
+                       “P(a:mem(Pow(N * X)))” 
+                       “IN(a:mem(Pow(N * X)),isLs(X))”)
+
+
+
+argQ = uexth |> concl
+
+
+
+new_spec
+“(!AB p1:AB->A p2:AB->B.
+ ?!i:AB->AB j. i o j = Id(AB) & j o i = Id(AB) &
+  p1 o i = p1 & p2 o i = p2 &
+  p1 o j = p1 & p2 o j = p2) &
+ (!AB p1:AB->A p2:AB->B AB' p1':AB'->A p2':AB'->B. 
+  (?!i:AB->AB' j. i o j = Id(AB') & j o i = Id(AB) &
+   p1' o i = p1 & p2' o i = p2 &
+   p1 o j = p1' & p2 o j = p2')==>
+  (?!i:AB'->AB j. i o j = Id(AB) & j o i = Id(AB') &
+   p1 o i = p1' & p2 o i = p2' &
+   p1' o j = p1 & p2' o j = p2)) & 
+ (!AB p1:AB->A p2:AB->B AB' p1':AB'->A p2':AB'->B
+      AB'' p1'':AB''->A p2'':AB''->B. 
+  (?!i:AB->AB' j. i o j = Id(AB') & j o i = Id(AB) &
+   p1' o i = p1 & p2' o i = p2 &
+   p1 o j = p1' & p2 o j = p2') &
+  (?!i:AB'->AB'' j. i o j = Id(AB'') & j o i = Id(AB') &
+   p1'' o i = p1' & p2'' o i = p2' &
+   p1' o j = p1'' & p2' o j = p2'') ==>
+  (?!i:AB->AB'' j. i o j = Id(AB'') & j o i = Id(AB) &
+   p1'' o i = p1 & p2'' o i = p2 &
+   p1 o j = p1'' & p2 o j = p2''))
+ ”)
+
+
+
 
 
 
@@ -326,3 +466,5 @@ uex_expand uexth0
 
 val argQ = (arg,Q);
 val arg12eqr = (arg1,arg2,eqr)
+*)
+*)
