newspecexpri.sml
@@ -1,0 +1,488 @@
+
+
+
+val isPair_def = qdefine_psym("isPair",[‘p1:AxB->A’,‘p2:AxB->B’])
+‘!x:mem(A) y:mem(B). 
+   ?!r:mem(AxB).App(p1,r) = x & App(p2,r) = y’
+
+val isPair_uex = prove_store("isPair_uex",
+e0
+(rpt gen_tac >> strip_tac (* 2 *)
+ >-- fs[isPair_def] >>
+     qby_tac
+     ‘∀ab:mem(AB).
+      ?!ab'. App(p1,ab) = App(p1',ab') & 
+             App(p2,ab) = App(p2',ab')’ 
+     >-- (strip_tac >> flip_tac >> arw[]) >>
+     drule
+     (P2fun |> qspecl [‘AB’,‘AB'’] 
+     |> fVar_sInst_th “P(ab:mem(AB),ab':mem(AB'))”
+        “App(p1:AB->A,ab) = App(p1':AB'->A,ab') & 
+         App(p2:AB->B,ab) = App(p2':AB'->B,ab')”) >>
+     pop_assum (x_choose_then "i" assume_tac) >>
+     qby_tac
+     ‘∀ab':mem(AB').
+      ?!ab. App(p1,ab) = App(p1',ab') & 
+             App(p2,ab) = App(p2',ab')’ 
+     >-- arw[] >>
+     drule
+     (P2fun |> qspecl [‘AB'’,‘AB’] 
+     |> fVar_sInst_th “P(ab':mem(AB'),ab:mem(AB))”
+        “App(p1:AB->A,ab) = App(p1':AB'->A,ab') & 
+         App(p2:AB->B,ab) = App(p2':AB'->B,ab')”) >> 
+     pop_assum (x_choose_then "j" assume_tac) >>
+     qexistsl_tac [‘i’,‘j’] >>
+     qby_tac
+     ‘i o j = Id(AB')’ 
+     >-- (arw[GSYM FUN_EXT,Id_def,App_App_o] >>
+         pop_assum (assume_tac o GSYM) >> arw[]) >>
+     qby_tac
+     ‘j o i = Id(AB)’ 
+     >-- (arw[GSYM FUN_EXT,Id_def,App_App_o] >>
+          strip_tac >>
+          last_x_assum (qsspecl_then [‘a’,‘App(i,a)’] (assume_tac o GSYM)) >>
+          arw[]) >>
+     arw[] >>
+     qby_tac
+     ‘p1' o i = p1 & p2' o i = p2’
+     >-- (arw[GSYM FUN_EXT,App_App_o] >> 
+         qpick_x_assum
+         ‘∀a b.
+          App(i, a) = b <=>
+          App(p1, a) = App(p1', b) & App(p2, a) = App(p2', b)’
+         (assume_tac o GSYM) >> flip_tac >> 
+         qsuff_tac
+         ‘∀a. App(p1,a) = App(p1',App(i,a)) &
+              App(p2,a) = App(p2',App(i,a))’ 
+         >-- (rpt strip_tac >> arw[]) >> arw[]) >> arw[] >>
+     arw[GSYM FUN_EXT,App_App_o] >> 
+     qpick_x_assum
+     ‘∀a b.
+      App(j, a) = b <=>
+      App(p1, b) = App(p1', a) & App(p2, b) = App(p2', a)’
+         (assume_tac o GSYM) >> 
+     qsuff_tac
+     ‘∀a. App(p1,App(j,a)) = App(p1',a) &
+          App(p2,App(j,a)) = App(p2',a)’ 
+     >-- (rpt strip_tac >> arw[]) >>
+     arw[])
+(form_goal “!A B AB p1:AB->A p2:AB ->B AB' p1':AB'->A p2'. 
+ isPair(p1,p2) & isPair(p1',p2') ⇒ 
+ ?i:AB->AB' j. i o j = Id(AB') & j o i = Id(AB) &
+  p1' o i = p1 & p2' o i = p2 &
+  p1 o j = p1' & p2 o j = p2'”));
+
+
+val Pr_uex = prove_store("Pr_uex",
+e0
+(rpt strip_tac >>
+ qspecl_then [‘A’,‘B’] assume_tac Cross_ex >>
+ pop_assum strip_assume_tac >>
+ qexistsl_tac [‘AxB’,‘p1’,‘p2’] >>
+ qby_tac
+ ‘isPair(p1,p2)’ 
+ >-- (rw[isPair_def] >>
+     rpt strip_tac >>
+     uex_tac >> first_x_assum (qspecl_then [‘x’,‘y’] strip_assume_tac) >>
+     qexists_tac ‘r’ >> arw[] >>
+     rpt strip_tac >> first_x_assum irule >> arw[]) >>
+ arw[] >> rpt strip_tac >>
+ qsspecl_then [‘p1’,‘p2’,‘p1'’,‘p2'’] assume_tac  isPair_uex >>
+ first_x_assum irule >> arw[])
+(form_goal “!A B. ?AB p1:AB->A p2:AB ->B. 
+ isPair(p1,p2) &
+ (!AB' p1':AB'->A p2'. isPair(p1',p2') ==>
+  ?i:AB->AB' j. i o j = Id(AB') & j o i = Id(AB) &
+  p1' o i = p1 & p2' o i = p2 &
+  p1 o j = p1' & p2 o j = p2')”));
+
+val Pr_ts_ex = proved_th $
+e0
+(rpt strip_tac >>
+ qspecl_then [‘A’,‘B’] strip_assume_tac Cross_ex >>
+ qexistsl_tac [‘AxB’,‘p1’,‘p2’] >> rw[])
+(form_goal “!A B. ?AB p1:AB->A p2:AB ->B. T”)
+
+val Reqv = proved_th $
+e0
+(rpt strip_tac (* 3 *)
+ >-- (qexistsl_tac [‘Id(AB)’,‘Id(AB)’] >> rw[IdL,IdR]) 
+ >-- (qexistsl_tac [‘j’,‘i’] >> arw[]) >>
+ qexistsl_tac [‘i' o i’,‘j o j'’] >>
+ arw[GSYM o_assoc] >>
+ qsuff_tac
+ ‘i' o (i o j) o j' = Id(AB'') & j o (j' o i') o i = Id(AB)’ 
+ >-- rw[o_assoc] >>
+ arw[IdL,IdR])
+(form_goal 
+“(!AB p1:AB->A p2:AB->B.
+ ?i:AB->AB j. i o j = Id(AB) & j o i = Id(AB) &
+  p1 o i = p1 & p2 o i = p2 &
+  p1 o j = p1 & p2 o j = p2) &
+ (!AB p1:AB->A p2:AB->B AB' p1':AB'->A p2':AB'->B. 
+  (?i:AB->AB' j. i o j = Id(AB') & j o i = Id(AB) &
+   p1' o i = p1 & p2' o i = p2 &
+   p1 o j = p1' & p2 o j = p2')==>
+  (?i:AB'->AB j. i o j = Id(AB) & j o i = Id(AB') &
+   p1 o i = p1' & p2 o i = p2' &
+   p1' o j = p1 & p2' o j = p2)) & 
+ (!AB p1:AB->A p2:AB->B AB' p1':AB'->A p2':AB'->B
+      AB'' p1'':AB''->A p2'':AB''->B. 
+  (?i:AB->AB' j. i o j = Id(AB') & j o i = Id(AB) &
+   p1' o i = p1 & p2' o i = p2 &
+   p1 o j = p1' & p2 o j = p2') &
+  (?i:AB'->AB'' j. i o j = Id(AB'') & j o i = Id(AB') &
+   p1'' o i = p1' & p2'' o i = p2' &
+   p1' o j = p1'' & p2' o j = p2'') ==>
+  (?i:AB->AB'' j. i o j = Id(AB'') & j o i = Id(AB) &
+   p1'' o i = p1 & p2'' o i = p2 &
+   p1 o j = p1'' & p2 o j = p2''))
+ ”)
+
+val uexth = Pr_uex |> spec_all
+
+val eth = Pr_ts_ex |> spec_all
+
+val eqvth = Reqv
+
+val fnames = ["*","p1","p2"]
+
+(*val iseqr = “P()”*)
+
+
+val arg1 = List.map (dest_var o rastt) 
+                    ["AB","p1:AB->A","p2:AB->B"]
+
+val arg2 = List.map (dest_var o rastt) 
+                     ["AB'","p1':AB'->A","p2':AB'->B"]
+
+val eqr = 
+“?i:AB->AB' j. i o j = Id(AB') & j o i = Id(AB) &
+   (p1':AB'->A) o i = p1 & (p2':AB'->B) o i = p2 &
+   p1 o j = p1' & p2 o j = p2'”
+
+
+val arg = arg1
+val Q = “isPair(p1:AB->A,p2:AB->B)”
+
+val argQ = (arg,Q)
+
+val vl = List.map dest_var [rastt "A",rastt "B"]
+
+
+val arg12eqr = (arg1,arg2,eqr)
+
+
+new_spec argQ arg12eqr ["*","p1","p2"] vl eth eqvth uexth
+
+
+
+
+val Id_uex = prove_store("Id_uex",
+e0
+(cheat)
+(form_goal “?i:A ->A. (!a.App(i,a) = a) & 
+ !i'. (!a.App(i',a) = a) ==> i = i'”));
+
+val uexth = Id_uex
+
+val eth = proved_th $
+e0
+cheat
+(form_goal “?i:A->A.T”)
+
+val vl = [("A",set_sort)]
+
+(*spec of new fsym if the input is a uex theorem with assumptions*)
+
+val fname = "Id"
+
+val argQ = ([dest_var (rastt "i:A->A")],“!a. App(i:A->A,a) = a”)
+
+val arg12eqr = ([dest_var (rastt "i:A->A")],[dest_var (rastt "i':A->A")],
+                “i = i':A->A”)
+
+val eqvth = proved_th $
+e0
+cheat
+(form_goal “(!i:A->A. i = i) &
+ (!i:A->A i':A->A. i = i' ==> i' = i) &
+ (!i:A->A i':A->A i'':A->A. 
+   i = i' & i' = i'' ==> i = i'')”)
+
+new_spec argQ arg12eqr [fname] vl eth eqvth uexth
+
+
+val Id_uex0 = prove_store("Id_uex0",
+e0
+(cheat)
+(form_goal “?!i:A ->A. (!a.App(i,a) = a)”));
+
+val uexth0 = Id_uex0
+
+simple_uex_spec "Id" [("A",set_sort)] Id_uex0
+
+
+
+set_spec (rastt "N0") sname iname fvs uexth
+
+
+
+
+val Exp_ev_unique = prove_store("Exp_ev_unique",
+e0
+(rpt strip_tac >> 
+ qby_tac
+ ‘∀a2b.?!a2b'.∀a. App(Ap1(ev,a2b),a) = App(ev',Pair(a,a2b'))’
+ >-- (strip_tac >>
+     first_x_assum (qsspecl_then [‘Ap1(ev,a2b)’] assume_tac) >>
+     flip_tac >> arw[]) >>
+ drule 
+ (P2fun |> qspecl [‘A2B’,‘A2B'’] 
+        |> fVar_sInst_th “P(a2b:mem(A2B),a2b':mem(A2B'))”
+           “∀a. App(Ap1(ev:A * A2B -> B,a2b),a) = 
+                App(ev':A * A2B' -> B,Pair(a,a2b'))”) >>
+ pop_assum (x_choose_then "i" assume_tac) >>
+ qby_tac
+ ‘∀a2b'.?!a2b.∀a. App(Ap1(ev',a2b'),a) = App(ev,Pair(a,a2b))’
+ >-- (strip_tac >>
+     first_x_assum (qsspecl_then [‘Ap1(ev',a2b')’] assume_tac) >>
+     flip_tac >> arw[]) >>
+ drule 
+ (P2fun |> qspecl [‘A2B'’,‘A2B’] 
+        |> fVar_sInst_th “P(a2b':mem(A2B'),a2b:mem(A2B))”
+           “∀a. App(Ap1(ev':A * A2B' -> B,a2b'),a) = 
+                App(ev:A * A2B -> B,Pair(a,a2b))”) >>
+ pop_assum (x_choose_then "j" assume_tac) >>
+ qexistsl_tac [‘i’,‘j’] >> 
+ qby_tac
+ ‘i o j = Id(A2B')’ 
+ >-- (rw[GSYM FUN_EXT,Id_def,App_App_o] >> arw[] >>
+     strip_tac >>
+     last_x_assum (qsspecl_then [‘a’,‘App(j,a)’] assume_tac) >>
+     fs[] >> 
+     pop_assum (assume_tac o GSYM) >> arw[Ap1_def]) >>
+ qby_tac
+ ‘j o i = Id(A2B)’ 
+ >-- (rw[GSYM FUN_EXT,Id_def,App_App_o] >> arw[] >>
+     strip_tac >>
+     first_x_assum (qsspecl_then [‘a’,‘App(i,a)’] assume_tac) >>
+     fs[] >> 
+     pop_assum (assume_tac o GSYM) >> arw[Ap1_def]) >>
+ arw[] >>
+ qby_tac
+ ‘ev' o Prla(Id(A), i) = ev’ 
+ >-- (rw[GSYM FUN_EXT] >> forall_cross_tac >> 
+     rw[App_App_o,App_Prla,Id_def] >>
+     fs[Ap1_def] >>
+     flip_tac >> rpt strip_tac >>
+     first_x_assum (irule o iffLR) >> rw[]) >>
+ qby_tac
+ ‘ev o Prla(Id(A), j) = ev'’ 
+ >-- (rw[GSYM FUN_EXT] >> forall_cross_tac >> 
+     rw[App_App_o,App_Prla,Id_def] >>
+     fs[Ap1_def] >>
+     flip_tac >> rpt strip_tac >>
+     first_x_assum (irule o iffLR) >> rw[]) >>
+ arw[])
+(form_goal 
+ “∀A B A2B ev:A * A2B ->B A2B' ev': A * A2B' -> B.
+  (!f:A->B.?!sf:mem(A2B).!a:mem(A).App(ev,Pair(a,sf)) = App(f,a)) &
+  (!f:A->B.?!sf:mem(A2B').!a:mem(A).App(ev',Pair(a,sf)) = App(f,a)) ⇒
+  ∃i: A2B -> A2B' j:A2B' -> A2B. 
+   i o j = Id(A2B') & j o i = Id(A2B) &
+   ev' o Prla(Id(A),i)  = ev & ev o Prla(Id(A),j) = ev'”));
+
+
+val Exp_ex_uex = prove_store("Exp_ex_uex",
+e0
+(rpt strip_tac >>
+ qspecl_then [‘A’,‘B’] strip_assume_tac Exp_ex >>
+ qexistsl_tac [‘A2B’,‘ev’] >> arw[] >> 
+ rpt strip_tac >> irule Exp_ev_unique >> arw[])
+(form_goal
+“!A B.
+ ?A2B ev:A * A2B ->B. 
+ (!f:A->B.?!sf:mem(A2B).!a:mem(A).App(ev,Pair(a,sf)) = App(f,a)) &
+ ∀A2B' ev':A * A2B' -> B.
+ (∀f:A->B.?!sf:mem(A2B').!a:mem(A).App(ev',Pair(a,sf)) = App(f,a)) ⇒
+ ∃i: A2B -> A2B' j:A2B' -> A2B. 
+   i o j = Id(A2B') & j o i = Id(A2B) &
+   ev' o Prla(Id(A),i)  = ev & ev o Prla(Id(A),j) = ev'”));
+
+val Exp_uex_refl = proved_th $
+e0
+(rpt strip_tac >> qexistsl_tac [‘Id(A2B)’,‘Id(A2B)’] >> 
+ rw[IdL,IdR,Prla_Id])
+(form_goal 
+ “∀A2B ev:A * A2B -> B.
+  ∃i: A2B -> A2B j:A2B -> A2B. 
+   i o j = Id(A2B) & j o i = Id(A2B) &
+   ev o Prla(Id(A),i)  = ev & ev o Prla(Id(A),j) = ev”)
+
+
+val Exp_uex_sym = proved_th $
+e0
+(rpt strip_tac >> qexistsl_tac [‘j’,‘i’] >> arw[])
+(form_goal 
+ “∀A2B ev:A * A2B -> B A2B' ev':A * A2B' -> B.
+  (∃i: A2B -> A2B' j:A2B' -> A2B. 
+   i o j = Id(A2B') & j o i = Id(A2B) &
+   ev' o Prla(Id(A),i)  = ev & ev o Prla(Id(A),j) = ev') ⇒ 
+  (∃i: A2B' -> A2B j:A2B -> A2B'.
+   i o j = Id(A2B) & j o i = Id(A2B') &
+   ev o Prla(Id(A),i) = ev' & ev' o Prla(Id(A),j) = ev)”)
+
+
+val Exp_uex_trans = proved_th $
+e0
+(rpt strip_tac >>
+ qexistsl_tac [‘i' o i’,‘j o j'’] >> 
+ rw[Prla_rsplit2] >> arw[GSYM o_assoc] >>
+ qsuff_tac
+ ‘i' o (i o j) o j' = Id(A2B'') & j o (j' o i') o i = Id(A2B)’
+ >-- rw[o_assoc] >>
+ arw[IdL,IdR])
+(form_goal 
+ “∀A2B ev:A * A2B -> B A2B' ev':A * A2B' -> B A2B'' ev'':A * A2B'' -> B.
+  (∃i: A2B -> A2B' j:A2B' -> A2B. 
+   i o j = Id(A2B') & j o i = Id(A2B) &
+   ev' o Prla(Id(A),i)  = ev & ev o Prla(Id(A),j) = ev') & 
+  (∃i: A2B' -> A2B'' j:A2B'' -> A2B'.
+   i o j = Id(A2B'') & j o i = Id(A2B') &
+   ev'' o Prla(Id(A),i) = ev' & ev' o Prla(Id(A),j) = ev'') ⇒ 
+  (∃i: A2B -> A2B'' j:A2B'' -> A2B.
+   i o j = Id(A2B'') & j o i = Id(A2B) &
+   ev'' o Prla(Id(A),i) = ev & ev o Prla(Id(A),j) = ev'')”)
+
+
+val Exp_ev_eqv = conjI Exp_uex_refl (conjI Exp_uex_sym Exp_uex_trans)
+
+val arg = [("A2B",set_sort),("ev",fun_sort (rastt "A * A2B") (rastt "B"))]
+
+val Q = “!f:A->B.?!sf:mem(A2B).!a:mem(A).App(ev,Pair(a,sf)) = App(f,a)”
+val argQ = (arg,Q) 
+
+val arg1 = arg 
+val arg2 = [("A2B'",set_sort),("ev'",fun_sort (rastt "A * A2B'") (rastt "B"))] 
+
+val eqr = “(∃i: A2B -> A2B' j:A2B' -> A2B. 
+   i o j = Id(A2B') & j o i = Id(A2B) &
+   ev' o Prla(Id(A),i)  = ev:A * A2B ->B & ev o Prla(Id(A),j) = ev')”
+
+val arg12eqr = (arg1,arg2,eqr) 
+val fnames = ["Exp","ev"]
+
+val vl = [("A",set_sort),("B",set_sort)] 
+
+
+val eth = proved_th $
+e0
+cheat
+(form_goal
+“?A2B ev:A * A2B ->B. T”)
+
+val eqvth = Exp_ev_eqv
+val uexth = Exp_ex_uex
+
+new_spec argQ arg12eqr fnames vl eth eqvth (spec_all uexth)
+
+check_ER arg12eqr eqvth uexth 
+
+val argseqr = arg12eqr
+
+val reflth = Exp_uex_refl
+
+
+
+val symth = Exp_uex_sym
+
+val transth = Exp_uex_trans
+
+
+fun check_ER argseqr eqvth uexth = 
+    let val eqvcls = mk_ER_condf argseqr
+        val _ = eq_form (eqvcls,concl eqvth) orelse
+                raise simple_fail "newspec.eqvth concl"
+        val _ = HOLset.isSubset(cont eqvth,cont uexth) orelse
+                raise simple_fail "newspec.eqvth cont"
+        val _ = List.all 
+                    (fn asm => 
+                        List.exists
+                            (fn a => eq_form(a,asm)) (ant uexth))
+                    (ant eqvth) orelse
+                raise simple_fail "newspec.eqvth ant"
+
+val Pow_unique = prove_store("Pow_unique",
+e0
+(cheat)
+(form_goal
+ “∀PA e:A ~>PA PA' e':A~> PA'.
+  (∀S1:1~>A. 
+   ?!s:mem(PA).
+     !x. Holds(S1,dot,x) ⇔ Holds(e,x,s)) &
+  (∀S1:1~>A. 
+   ?!s:mem(PA').
+     !x. Holds(S1,dot,x) ⇔ Holds(e',x,s)) ⇒
+  ∃i:PA -> PA' j:PA' -> PA. 
+     i o j = Id(PA') & j o i = Id(PA) &
+     asR(i) @ e = e' & asR(j) @ e' = e ”));
+
+val Pow_R_REFL = prove_store("Pow_R_REFL",
+e0
+(rpt strip_tac >> qexistsl_tac [‘Id(PA)’,‘Id(PA)’] >>
+ rw[IdL,IdR,asR_Id,idL,idR])
+(form_goal
+ “∀PA e:A ~>PA.
+    ∃i:PA -> PA j:PA -> PA. 
+     i o j = Id(PA) & j o i = Id(PA) &
+     asR(i) @ e = e & asR(j) @ e = e ”));
+
+
+val Pow_R_SYM = prove_store("Pow_R_SYM",
+e0
+(rpt strip_tac >>
+ qexistsl_tac [‘j’,‘i’] >> arw[])
+(form_goal
+ “∀PA e:A~>PA PA' e':A~> PA'.
+(∃i:PA -> PA' j:PA' -> PA. 
+   i o j = Id(PA') & j o i = Id(PA) &
+   asR(i) @ e = e' & asR(j) @ e' = e) ⇒
+ (∃i:PA' -> PA j:PA -> PA'. 
+   i o j = Id(PA) & j o i = Id(PA') &
+   asR(i) @ e' = e & asR(j) @ e = e')”));
+
+
+val Pow_R_TRANS = prove_store("Pow_R_TRANS",
+e0
+(rpt strip_tac >>
+ qexistsl_tac [‘i' o i’,‘j o j'’] >> 
+ arw[ao_assoc,asR_o]>>
+ qsuff_tac
+ ‘i' o (i o j) o j' = Id(PA'') & j o (j' o i') o i = Id(PA)’ 
+ >-- rw[o_assoc] >>
+ arw[IdR,IdL])
+(form_goal
+ “∀PA e:A~>PA PA' e':A~> PA' PA'' e'':A~>PA''.
+(∃i:PA -> PA' j:PA' -> PA. 
+   i o j = Id(PA') & j o i = Id(PA) &
+   asR(i) @ e = e' & asR(j) @ e' = e) &
+ (∃i:PA' -> PA'' j:PA'' -> PA'. 
+   i o j = Id(PA'') & j o i = Id(PA') &
+   asR(i) @ e' = e'' & asR(j) @ e'' = e') ⇒
+ (∃i:PA -> PA'' j:PA'' -> PA. 
+   i o j = Id(PA'') & j o i = Id(PA) &
+   asR(i) @ e = e'' & asR(j) @ e'' = e)”));
+
+
+val o_uex = prove_store("o_uex",
+e0
+(rpt strip_tac >> uex_tac >>
+ qsspecl_then [‘phi’,‘psi’] strip_assume_tac o_ex >>
+ qexists_tac ‘f’ >> arw[] >>
+ rpt strip_tac >> rw[GSYM FUN_EXT] >>
+ arw[] >> strip_tac >>  
+ last_x_assum (irule o iffLR) >> rw[])
+(form_goal
+ “!A B phi:A->B C psi:B->C. ?!f:A->C. 
+ !a c. App(f,a) = c <=> Holds(asR(psi) @ asR(phi),a,c)”));
